src/Ex/Mesi/MesiInvExcl.v
@@ -20,6 +20,21 @@ Local Open Scope fmap.
 
 Existing Instance Mesi.ImplOStateIfc.
 
+Definition NoCohMsgs (oidx: IdxT) (msgs: MessagePool Msg) :=
+  MsgsNotExist [(downTo oidx, (MRs, mesiRsS));
+               (downTo oidx, (MRs, mesiRsE));
+               (downTo oidx, (MRs, mesiRsM));
+               (rsUpFrom oidx, (MRs, mesiDownRsS));
+               (rsUpFrom oidx, (MRs, mesiDownRsIM))] msgs.
+
+Definition ObjInvalid0 (oidx: IdxT) (ost: OState) (msgs: MessagePool Msg) :=
+  ost#[status] <= mesiI /\
+  ost#[dir].(dir_st) <> mesiS /\
+  NoCohMsgs oidx msgs.
+
+Definition ObjInvalid (oidx: IdxT) (ost: OState) (msgs: MessagePool Msg) :=
+  ObjInvalid0 oidx ost msgs \/ ObjInvRs oidx msgs.
+
 Definition ObjsInvalid (inP: IdxT -> Prop) (oss: OStates) (msgs: MessagePool Msg) :=
   forall oidx,
     inP oidx ->
@@ -217,6 +232,25 @@ Section Facts.
     - eapply NoRsI_MsgExistsSig_InvRs_false; eauto.
   Qed.
 
+  Lemma ObjsInvalid_obj_dir_false:
+    forall inP oss msgs,
+      ObjsInvalid inP oss msgs ->
+      forall oidx,
+        inP oidx ->
+        NoRsI oidx msgs ->
+        forall ost,
+          oss@[oidx] = Some ost ->
+          ost#[dir].(dir_st) = mesiS ->
+          False.
+  Proof.
+    intros.
+    specialize (H _ H0).
+    rewrite H2 in H; simpl in H.
+    destruct H.
+    - red in H; solve_mesi.
+    - eapply NoRsI_MsgExistsSig_InvRs_false; eauto.
+  Qed.
+
   Lemma ObjsInvalid_this_state_silent:
     forall inP oss msgs,
       ObjsInvalid inP oss msgs ->
@@ -245,8 +279,8 @@ Section Facts.
     destruct (oss@[oidx]) as [ost|]; simpl in H; simpl; auto.
     destruct H.
     - left.
-      destruct H.
-      split; [assumption|dest_in; solve_MsgsP].
+      destruct H as [? [? ?]].
+      repeat split; [assumption..|dest_in; solve_MsgsP].
     - right.
       destruct H as [[rmidx rmsg] [? ?]]; inv H3.
       exists (downTo oidx, rmsg); split.
@@ -269,8 +303,8 @@ Section Facts.
     destruct (oss@[oidx]) as [ost|]; simpl in H; simpl; auto.
     destruct H.
     - left.
-      destruct H.
-      split; [assumption|dest_in; solve_MsgsP].
+      destruct H as [? [? ?]].
+      repeat split; [assumption..|dest_in; solve_MsgsP].
     - right.
       destruct H as [[rmidx msg] [? ?]]; inv H3.
       exists (downTo oidx, msg); split.
@@ -299,9 +333,9 @@ Section Facts.
     rewrite H0 in H; simpl in H.
     destruct H.
     - red in H; dest.
-      specialize (H6 (downTo oidx, rsdm) H3).
-      red in H6; rewrite map_trans, map_cons in H6.
-      rewrite caseDec_head_eq in H6
+      specialize (H7 (downTo oidx, rsdm) H3).
+      red in H7; rewrite map_trans, map_cons in H7.
+      rewrite caseDec_head_eq in H7
         by (unfold sigOf; simpl; congruence).
       auto.
     - destruct H as [[midx msg] [? ?]]; simpl in *.
@@ -330,13 +364,13 @@ Section Facts.
     rewrite H0 in H; simpl in H.
     destruct H.
     - red in H; dest.
-      specialize (H6 (downTo oidx, rsdm) H3).
-      red in H6; rewrite map_trans, map_cons in H6.
-      rewrite caseDec_head_neq in H6
+      specialize (H7 (downTo oidx, rsdm) H3).
+      red in H7; rewrite map_trans, map_cons in H7.
+      rewrite caseDec_head_neq in H7
         by (unfold sigOf; simpl; intro Hx; inv Hx;
-            rewrite H5 in H9; discriminate).
-      rewrite map_cons in H6.
-      rewrite caseDec_head_eq in H6
+            rewrite H5 in H10; discriminate).
+      rewrite map_cons in H7.
+      rewrite caseDec_head_eq in H7
         by (unfold sigOf; simpl; congruence).
       auto.
     - destruct H as [[midx msg] [? ?]]; simpl in *.
@@ -365,13 +399,13 @@ Section Facts.
     rewrite H0 in H; simpl in H.
     destruct H.
     - red in H; dest.
-      specialize (H6 (downTo oidx, rsdm) H3).
-      red in H6; rewrite map_trans, map_cons in H6.
-      do 2 (rewrite caseDec_head_neq in H6
+      specialize (H7 (downTo oidx, rsdm) H3).
+      red in H7; rewrite map_trans, map_cons in H7.
+      do 2 (rewrite caseDec_head_neq in H7
              by (unfold sigOf; simpl; intro Hx; inv Hx;
-                 rewrite H5 in H9; discriminate);
-            rewrite map_cons in H6).
-      rewrite caseDec_head_eq in H6
+                 rewrite H5 in H10; discriminate);
+            rewrite map_cons in H7).
+      rewrite caseDec_head_eq in H7
         by (unfold sigOf; simpl; congruence).
       auto.
     - destruct H as [[midx msg] [? ?]]; simpl in *.
@@ -400,13 +434,13 @@ Section Facts.
     rewrite H0 in H; simpl in H.
     destruct H.
     - red in H; dest.
-      specialize (H6 (rsUpFrom oidx, rsum) H3).
-      red in H6; rewrite map_trans, map_cons in H6.
-      do 3 (rewrite caseDec_head_neq in H6
+      specialize (H7 (rsUpFrom oidx, rsum) H3).
+      red in H7; rewrite map_trans, map_cons in H7.
+      do 3 (rewrite caseDec_head_neq in H7
              by (unfold sigOf; simpl; intro Hx; inv Hx;
                  rewrite H5 in H9; discriminate);
-            rewrite map_cons in H6).
-      rewrite caseDec_head_eq in H6
+            rewrite map_cons in H7).
+      rewrite caseDec_head_eq in H7
         by (unfold sigOf; simpl; congruence).
       auto.
     - destruct H as [[midx msg] [? ?]]; simpl in *.
@@ -415,7 +449,7 @@ Section Facts.
       eapply (H12 (rsUpFrom oidx, rsum)); eauto.
   Qed.
 
-  Lemma ObjsInvalid_downRsI_false:
+  Lemma ObjsInvalid_downRsIM_false:
     forall inP oss msgs,
       ObjsInvalid inP oss msgs ->
       forall oidx ost orq,
@@ -425,7 +459,7 @@ Section Facts.
         forall rsum,
           InMP (rsUpFrom oidx) rsum msgs ->
           rsum.(msg_type) = MRs ->
-          rsum.(msg_id) = mesiDownRsI ->
+          rsum.(msg_id) = mesiDownRsIM ->
           False.
   Proof.
     intros.
@@ -433,13 +467,13 @@ Section Facts.
     rewrite H0 in H; simpl in H.
     destruct H.
     - red in H; dest.
-      specialize (H6 (rsUpFrom oidx, rsum) H3).
-      red in H6; rewrite map_trans, map_cons in H6.
-      do 4 (rewrite caseDec_head_neq in H6
+      specialize (H7 (rsUpFrom oidx, rsum) H3).
+      red in H7; rewrite map_trans, map_cons in H7.
+      do 4 (rewrite caseDec_head_neq in H7
              by (unfold sigOf; simpl; intro Hx; inv Hx;
-                 rewrite H5 in H9; discriminate);
-            rewrite map_cons in H6).
-      rewrite caseDec_head_eq in H6
+                 rewrite H5 in H10; discriminate);
+            rewrite map_cons in H7).
+      rewrite caseDec_head_eq in H7
         by (unfold sigOf; simpl; congruence).
       auto.
     - destruct H as [[midx msg] [? ?]]; simpl in *.
@@ -452,8 +486,7 @@ Section Facts.
     forall msgs oidx,
       NoCohMsgs oidx msgs ->
       forall midx msg,
-        ~ In msg.(msg_id) [mesiRsS; mesiRsE; mesiRsM;
-                             mesiDownRsS; mesiDownRsI] ->
+        ~ In msg.(msg_id) [mesiRsS; mesiRsE; mesiRsM; mesiDownRsS; mesiDownRsIM] ->
         NoCohMsgs oidx (enqMP midx msg msgs).
   Proof.
     intros; apply MsgsP_other_msg_id_enqMP; assumption.
@@ -499,6 +532,30 @@ Section Facts.
     all: try (destruct H8 as [rsUp [? ?]]; inv H8;
               apply H6 with (rsUp:= rsUp); auto;
               eapply InMP_deqMP; eauto).
+  Qed.
+
+  Lemma NoCohMsgs_rsUp_in:
+    forall oidx msgs rmsg,
+      InMP (rsUpFrom oidx) rmsg msgs ->
+      rmsg.(msg_id) <> mesiDownRsS ->
+      rmsg.(msg_id) <> mesiDownRsIM ->
+      forall orq,
+        RsDownConflicts oidx orq msgs ->
+        RsUpConflicts oidx msgs ->
+        NoCohMsgs oidx msgs.
+  Proof.
+    intros.
+    specialize (H3 (rsUpFrom oidx, rmsg) eq_refl H); dest.
+    apply not_MsgExistsSig_MsgsNotExist.
+    intros; dest_in.
+    all: try (destruct H7 as [[midx msg] [? ?]]; inv H7;
+              specialize (H2 (downTo oidx, msg) eq_refl H10 H6); dest;
+              eapply H13 with (rsUp:= (rsUpFrom oidx, rmsg)); eauto; fail).
+    all: (destruct H7 as [[midx msg] [? ?]]; inv H7;
+          eapply H4;
+          eapply findQ_length_two; [|apply H|apply H6];
+          simpl; intro Hx; subst;
+          congruence).
   Qed.
 
   Lemma NoCohMsgs_rsUp_deq:
@@ -556,27 +613,31 @@ Section Facts.
       forall oidx orq,
         inP oidx ->
         RsDownConflicts oidx orq msgs ->
-        forall nost: OState,
-          nost#[status] = mesiNP ->
-          nost#[owned] = false ->
-          forall rmsg,
-            FirstMPI msgs (downTo oidx, rmsg) ->
-            rmsg.(msg_type) = MRs ->
-            ObjsInvalid inP (oss +[ oidx <- nost]) (deqMP (downTo oidx) msgs).
+        forall post,
+          oss@[oidx] = Some post ->
+          forall nost: OState,
+            nost#[status] = mesiNP ->
+            nost#[dir].(dir_st) = mesiI -> (* by [InvWBDir] *)
+            nost#[owned] = false ->
+            forall rmsg,
+              FirstMPI msgs (downTo oidx, rmsg) ->
+              rmsg.(msg_type) = MRs ->
+              ObjsInvalid inP (oss +[ oidx <- nost]) (deqMP (downTo oidx) msgs).
   Proof.
     intros.
     red; intros roidx ?.
-    specialize (H _ H6).
-    mred; simpl in *; auto.
-    - left; split.
+    mred; simpl in *.
+    - left; repeat split.
       + simpl; solve_mesi.
+      + simpl; rewrite H4; discriminate.
       + eapply NoCohMsgs_rsDown_deq; eauto.
-    - destruct (oss@[roidx]) as [rost|]; simpl in *; auto.
+    - specialize (H _ H8).
+      destruct (oss@[roidx]) as [rost|]; simpl in *; auto.
       destruct H; [left|right].
-      + destruct H; split; [assumption|].
+      + destruct H as [? [? ?]]; repeat split; [assumption..|].
         solve_MsgsP.
       + destruct H as [[midx msg] [? ?]].
-        exists (midx, msg); split; [|assumption]; inv H7.
+        exists (midx, msg); split; [|assumption]; inv H9.
         apply deqMP_InMP_midx; [assumption|].
         simpl; intro Hx; subst.
         inv Hx; auto.
@@ -679,8 +740,8 @@ Section Facts.
       destruct (oss@[oidx]) as [ost|]; simpl in H; simpl; auto.
       destruct H.
       - left.
-        destruct H.
-        split; [assumption|dest_in; solve_MsgsP].
+        destruct H as [? [? ?]].
+        repeat split; [assumption..|dest_in; solve_MsgsP].
       - right.
         destruct H as [[rmidx msg] [? ?]]; inv H3.
         exists (downTo oidx, msg); split.
@@ -691,13 +752,14 @@ Section Facts.
         + unfold sigOf; simpl; congruence.
     Qed.
 
-    Lemma ObjsInvalid_rsE_consumed:
+    Lemma ObjsInvalid_rsDown_invalidated:
       forall oss msgs oidx orq,
         ObjsInvalid (fun idx => oidx <> idx) oss msgs ->
         RsDownConflicts oidx orq msgs ->
         forall cidx (nost: OState) rmsg,
           parentIdxOf topo cidx = Some oidx ->
           nost#[status] = mesiI ->
+          nost#[dir].(dir_st) <> mesiS ->
           FirstMPI msgs (downTo oidx, rmsg) ->
           rmsg.(msg_type) = MRs ->
           ObjsInvalid (fun idx => cidx <> idx)
@@ -706,15 +768,17 @@ Section Facts.
     Proof.
       intros; subst topo.
       red; intros; mred.
-      - simpl; left; split; [simpl in *; solve_mesi|].
-        eapply NoCohMsgs_rsDown_deq; eauto.
+      - simpl; left; repeat split.
+        + simpl in *; solve_mesi.
+        + assumption.
+        + eapply NoCohMsgs_rsDown_deq; eauto.
       - specialize (H _ (neq_sym n)).
         destruct (oss@[oidx0]) as [ost|]; simpl in *; auto.
         destruct H; [left|right].
-        + destruct H; split; [assumption|].
-          solve_MsgsP.
+        + destruct H as [? [? ?]].
+          repeat split; [assumption..|solve_MsgsP].
         + destruct H as [[midx msg] [? ?]].
-          exists (midx, msg); split; [|assumption]; inv H6.
+          exists (midx, msg); split; [|assumption]; inv H7.
           apply deqMP_InMP_midx; [assumption|].
           simpl; intro Hx; subst.
           inv Hx; auto.
@@ -727,13 +791,17 @@ Section Facts.
         forall cidx (nost: OState),
           parentIdxOf topo cidx = Some oidx ->
           nost#[status] = mesiI ->
+          nost#[dir].(dir_st) = mesiE ->
           ObjsInvalid (fun idx => cidx <> idx)
                       (oss +[oidx <- nost])
                       msgs.
     Proof.
       intros; subst topo.
       red; intros; mred; auto.
-      simpl; left; split; [simpl in *; solve_mesi|assumption].
+      simpl; left; repeat split.
+      - simpl in *; solve_mesi.
+      - rewrite H3; discriminate.
+      - assumption.
     Qed.
 
     Lemma ObjsInvalid_rsM_consumed:
@@ -745,6 +813,7 @@ Section Facts.
         InvDirInv topo cifc oidx ost oss msgs ->
         forall cidx (nost: OState) rmsg,
           nost#[status] = mesiI ->
+          nost#[dir].(dir_st) = mesiM ->
           FirstMPI msgs (downTo oidx, rmsg) ->
           rmsg.(msg_type) = MRs ->
           ObjsInvalid (fun idx => ~ In idx (subtreeIndsOf topo cidx))
@@ -753,24 +822,26 @@ Section Facts.
     Proof.
       intros; subst topo.
       red; intros; mred.
-      - simpl; left; split; [simpl in *; solve_mesi|].
-        eapply NoCohMsgs_rsDown_deq; eauto.
+      - simpl; left; repeat split.
+        + simpl in *; solve_mesi.
+        + rewrite H5; discriminate.
+        + eapply NoCohMsgs_rsDown_deq; eauto.
       - destruct (in_dec idx_dec oidx0 (subtreeIndsOf (fst (tree2Topo tr 0)) oidx)).
         + apply subtreeIndsOf_composed in i; auto.
           destruct i; [exfalso; auto|].
-          destruct H8 as [rcidx [? ?]].
+          destruct H9 as [rcidx [? ?]].
 
           (* Discharge [InvDirInv] *)
-          specialize (H3 H _ H8); destruct H3 as [? _].
+          specialize (H3 H _ H9); destruct H3 as [? _].
           specialize (H3 (getDir_st_I _ H2 _)).
-          specialize (H3 _ H9).
+          specialize (H3 _ H10).
 
           destruct (oss@[oidx0]) as [ost0|]; simpl in *; auto.
           destruct H3; [left|right].
-          * destruct H3; split; [assumption|].
-            solve_MsgsP.
+          * destruct H3 as [? [? ?]].
+            repeat split; [assumption..|solve_MsgsP].
           * destruct H3 as [[midx msg] [? ?]].
-            exists (midx, msg); split; [|assumption]; inv H10.
+            exists (midx, msg); split; [|assumption]; inv H11.
             apply deqMP_InMP_midx; [assumption|].
             simpl; intro Hx; subst.
             inv Hx; auto.
@@ -778,10 +849,10 @@ Section Facts.
         + specialize (H0 _ n0).
           destruct (oss@[oidx0]) as [ost0|]; simpl in *; auto.
           destruct H0; [left|right].
-          * destruct H0; split; [assumption|].
-            solve_MsgsP.
+          * destruct H0 as [? [? ?]].
+            repeat split; [assumption..|solve_MsgsP].
           * destruct H0 as [[midx msg] [? ?]].
-            exists (midx, msg); split; [|assumption]; inv H8.
+            exists (midx, msg); split; [|assumption]; inv H9.
             apply deqMP_InMP_midx; [assumption|].
             simpl; intro Hx; subst.
             inv Hx; auto.
@@ -794,16 +865,65 @@ Section Facts.
         forall cidx (nost: OState),
           parentIdxOf topo cidx = Some oidx ->
           nost#[status] = mesiI ->
+          nost#[dir].(dir_st) <> mesiS ->
           ObjsInvalid (fun idx => ~ In idx (subtreeIndsOf topo cidx))
                       (oss +[oidx <- nost])
                       msgs.
     Proof.
       intros; subst topo.
       red; intros; mred; auto.
-      simpl; left; split; [simpl in *; solve_mesi|assumption].
+      simpl; left; repeat split.
+      - simpl in *; solve_mesi.
+      - assumption.
+      - assumption.
     Qed.
 
-    Lemma ObjsInvalid_downRsI:
+    Lemma ObjsInvalid_downRsIS:
+      forall oss msgs oidx (ost: OState) orq,
+        In oidx (c_li_indices cifc) ->
+        RqDownConflicts oidx msgs ->
+        RsDownConflicts oidx orq msgs ->
+        ost#[dir].(dir_st) = mesiI ->
+        InvDirInv topo cifc oidx ost oss msgs ->
+        forall (nost: OState) rqm rsm,
+          nost#[status] = mesiI ->
+          nost#[dir].(dir_st) = mesiI ->
+          FirstMPI msgs (downTo oidx, rqm) ->
+          rqm.(msg_type) = MRq ->
+          rsm.(msg_id) = mesiDownRsIS ->
+          ObjsInvalid
+            (fun idx => In idx (subtreeIndsOf topo oidx))
+            (oss +[oidx <- nost])
+            (enqMP (rsUpFrom oidx) rsm (deqMP (downTo oidx) msgs)).
+    Proof.
+      intros; subst topo.
+      red; intros; mred.
+      - simpl; left; repeat split; [solve_mesi| |].
+        + rewrite H5; discriminate.
+        + apply NoCohMsgs_enq; [|rewrite H8; solve_not_in].
+          eapply NoCohMsgs_rqDown_deq; eauto.
+      - apply subtreeIndsOf_composed in H9; auto.
+        destruct H9; [exfalso; auto|].
+        destruct H9 as [cidx [? ?]].
+        destruct (oss@[oidx0]) as [ost0|] eqn:Host; simpl; auto.
+
+        (* Discharge [InvDirInv] *)
+        specialize (H3 H _ H9); destruct H3 as [? _].
+        specialize (H3 (getDir_st_I _ H2 _)).
+        specialize (H3 _ H10).
+
+        rewrite Host in H3; simpl in H3.
+        destruct H3; [left|right].
+        + destruct H3 as [? [? ?]]; repeat split; [assumption..|].
+          solve_MsgsP.
+        + destruct H3 as [[midx msg] [? ?]].
+          exists (midx, msg); split; [|assumption]; inv H11.
+          apply InMP_or_enqMP; right.
+          apply deqMP_InMP_midx; [assumption|].
+          simpl; intro Hx; inv Hx; auto.
+    Qed.
+
+    Lemma ObjsInvalid_downRsIM:
       forall oss msgs oidx (ost: OState) orq,
         In oidx (c_li_indices cifc) ->
         RqDownConflicts oidx msgs ->
@@ -814,7 +934,7 @@ Section Facts.
           nost#[status] = mesiI ->
           FirstMPI msgs (downTo oidx, rqm) ->
           rqm.(msg_type) = MRq ->
-          rsm.(msg_id) = mesiDownRsI ->
+          rsm.(msg_id) = mesiDownRsIM ->
           ObjsInvalid
             (fun idx =>
                exists cidx,
@@ -838,7 +958,7 @@ Section Facts.
 
         rewrite Host in H3; simpl in H3.
         destruct H3; [left|right].
-        + destruct H3; split; [assumption|].
+        + destruct H3 as [? [? ?]]; repeat split; [assumption..|].
           solve_MsgsP.
         + destruct H3 as [[midx msg] [? ?]].
           exists (midx, msg); split; [|assumption]; inv H10.
@@ -907,7 +1027,7 @@ Section Facts.
         apply H1; eauto.
     Qed.
 
-    Lemma ObjsInvalid_downRsI_composed:
+    Lemma ObjsInvalid_downRsIM_composed:
       forall oidx oss msgs ost,
         oss@[oidx] = Some ost ->
         (forall rcidx,
@@ -986,7 +1106,7 @@ Section InvExcl.
     forall oidx, ObjInvalid oidx implOStateInit (emptyMP Msg).
   Proof.
     intros; left.
-    split; [simpl; solve_mesi|].
+    repeat split; [simpl; solve_mesi|simpl; solve_mesi|].
     do 3 red; intros.
     do 2 red in H; dest_in.
   Qed.
@@ -1322,12 +1442,22 @@ Section InvExcl.
     (valOf eout).(msg_id) = mesiDownRsS ->
     ost <+- oss@[oidx]; (ost#[status] <= mesiS /\ ost#[owned] = false).
 
-  Definition DownRsIPred (oidx: IdxT) (eout: Id Msg) (oss: OStates)
+  Definition DownRsISPred (oidx: IdxT) (eout: Id Msg) (oss: OStates)
              (msgs: MessagePool Msg): Prop :=
     idOf eout = rsUpFrom oidx ->
     (valOf eout).(msg_type) = MRs ->
-    (valOf eout).(msg_id) = mesiDownRsI ->
+    (valOf eout).(msg_id) = mesiDownRsIS ->
     (ost <+- oss@[oidx]; ost#[status] = mesiI /\ ost#[owned] = false) /\
+    ObjsInvalid (fun idx => In idx (subtreeIndsOf topo oidx)) oss msgs.
+
+  Definition DownRsIMPred (oidx: IdxT) (eout: Id Msg) (oss: OStates)
+             (msgs: MessagePool Msg): Prop :=
+    idOf eout = rsUpFrom oidx ->
+    (valOf eout).(msg_type) = MRs ->
+    (valOf eout).(msg_id) = mesiDownRsIM ->
+    (ost <+- oss@[oidx]; ost#[status] = mesiI /\
+                         ost#[dir].(dir_st) = mesiI /\
+                         ost#[owned] = false) /\
     ObjsInvalid
       (fun idx =>
          exists cidx,
@@ -1353,7 +1483,8 @@ Section InvExcl.
       forall oidx,
         GetRqPred oidx eout /\ SetRqPred oidx eout /\
         RsMPred oidx eout oss msgs /\ RsEPred oidx eout oss msgs /\
-        DownRsSPred oidx eout oss msgs /\ DownRsIPred oidx eout oss msgs /\
+        DownRsSPred oidx eout oss msgs /\
+        DownRsISPred oidx eout oss msgs /\ DownRsIMPred oidx eout oss msgs /\
         InvRqPred oidx eout oss msgs /\ InvWRqPred oidx eout oss msgs.
 
   Lemma InvExclMsgOutPred_good:
@@ -1367,7 +1498,7 @@ Section InvExcl.
       do 2 (red; intros).
       specialize (H2 oidx0); dest.
       repeat ssplit;
-        try (red; intros; rewrite H11 in H1;
+        try (red; intros; rewrite H12 in H1;
              derive_child_chns oidx; disc_rule_conds_ex; fail).
 
     - red; intros; destruct H.
@@ -1376,33 +1507,31 @@ Section InvExcl.
       do 2 (red; intros).
       specialize (H4 oidx0); dest.
       repeat ssplit;
-        try (red; intros; rewrite H13 in H0;
+        try (red; intros; rewrite H14 in H0;
              derive_child_chns oidx; disc_rule_conds_ex; fail).
 
       + (* [DownRsSPred] *)
-        red; intros; rewrite H13 in H0.
+        red; intros; rewrite H14 in H0.
         derive_child_chns oidx; disc_rule_conds_ex.
         assert (In oidx (subtreeIndsOf (fst (tree2Topo tr 0)) oidx))
           by (eapply rqEdgeUpFrom_subtreeIndsOf_self_in;
               [eauto|congruence]).
-        pose proof (H5 _ H16); dest.
-        rewrite <-H17; apply H9; assumption.
+        pose proof (H5 _ H17); dest.
+        rewrite <-H18; apply H9; assumption.
 
-      + (* [DownRsIPred] *)
-        red; intros; rewrite H13 in H0.
+      + (* [DownRsISPred] *)
+        red; intros; rewrite H14 in H0.
         derive_child_chns oidx; disc_rule_conds_ex.
         split.
         * assert (In oidx (subtreeIndsOf (fst (tree2Topo tr 0)) oidx))
             by (eapply rqEdgeUpFrom_subtreeIndsOf_self_in;
                 [eauto|congruence]).
-          pose proof (H5 _ H16); dest.
-          rewrite <-H17; apply H10; assumption.
+          pose proof (H5 _ H17); dest.
+          rewrite <-H18; apply H10; assumption.
         * red; intros.
-          specialize (H10 H13 H14 H15); destruct H10 as [? ?].
-          specialize (H17 _ H16).
-          destruct H16 as [cidx [? ?]].
-          eapply subtreeIndsOf_child_SubList in H18; eauto.
-          specialize (H5 _ H18); dest.
+          specialize (H10 H14 H15 H16); destruct H10 as [? ?].
+          specialize (H18 _ H17).
+          specialize (H5 _ H17); dest.
           rewrite <-H5.
           assert (exists pidx0, parentIdxOf (fst (tree2Topo tr 0)) oidx0 = Some pidx0).
           { eapply subtreeIndsOf_in_has_parent with (oidx:= oidx); eauto. }
@@ -1414,18 +1543,60 @@ Section InvExcl.
           specialize (H25 _ H23).
           specialize (H26 _ H24).
           destruct (oss1@[oidx0]) as [ost0|]; simpl in *; auto.
-          destruct H17; [left|right].
-          { destruct H17; split; [assumption|].
+          destruct H18; [left|right].
+          { destruct H18 as [? [? ?]].
+            repeat split; [assumption..|].
             apply not_MsgExistsSig_MsgsNotExist; intros.
-            eapply MsgExistsSig_MsgsNotExist_false in H27; eauto.
+            eapply MsgExistsSig_MsgsNotExist_false in H29; eauto.
             dest_in.
-            all: try (destruct H29 as [[midx msg] [? ?]];
-                      exists (midx, msg); split; [|assumption]; inv H29;
-                      do 2 red in H28; do 2 red; simpl in *; congruence).
+            all: try (destruct H30 as [[midx msg] [? ?]];
+                      exists (midx, msg); split; [|assumption]; inv H30;
+                      do 2 red in H29; do 2 red; simpl in *; congruence).
           }
-          { destruct H17 as [[midx msg] [? ?]].
+          { destruct H18 as [[midx msg] [? ?]].
             exists (midx, msg); split; [|assumption]; inv H27.
-            do 2 red in H17; do 2 red; simpl in *; congruence.
+            do 2 red in H18; do 2 red; simpl in *; congruence.
+          }
+
+      + (* [DownRsIMPred] *)
+        red; intros; rewrite H14 in H0.
+        derive_child_chns oidx; disc_rule_conds_ex.
+        split.
+        * assert (In oidx (subtreeIndsOf (fst (tree2Topo tr 0)) oidx))
+            by (eapply rqEdgeUpFrom_subtreeIndsOf_self_in;
+                [eauto|congruence]).
+          pose proof (H5 _ H17); dest.
+          rewrite <-H18; apply H11; assumption.
+        * red; intros.
+          specialize (H11 H14 H15 H16); destruct H11 as [? ?].
+          specialize (H18 _ H17).
+          destruct H17 as [cidx [? ?]].
+          eapply subtreeIndsOf_child_SubList in H19; eauto.
+          specialize (H5 _ H19); dest.
+          rewrite <-H5.
+          assert (exists pidx0, parentIdxOf (fst (tree2Topo tr 0)) oidx0 = Some pidx0).
+          { eapply subtreeIndsOf_in_has_parent with (oidx:= oidx); eauto. }
+          destruct H22 as [pidx0 ?].
+          derive_child_chns oidx0.
+
+          red in H21; dest.
+          specialize (H21 _ H23).
+          specialize (H26 _ H24).
+          specialize (H27 _ H25).
+          destruct (oss1@[oidx0]) as [ost0|]; simpl in *; auto.
+          destruct H18; [left|right].
+          { destruct H18 as [? [? ?]].
+            repeat split; [assumption..|].
+            apply not_MsgExistsSig_MsgsNotExist; intros.
+            eapply MsgExistsSig_MsgsNotExist_false in H30; eauto.
+            dest_in.
+            all: try (destruct H31 as [[midx msg] [? ?]];
+                      exists (midx, msg); split; [|assumption]; inv H31;
+                      do 2 red in H30; do 2 red; simpl in *; congruence).
+          }
+          { destruct H18 as [[midx msg] [? ?]].
+            exists (midx, msg); split; [|assumption]; inv H28.
+            do 2 red in H18; do 2 red; simpl in *; congruence.
           }
   Qed.
   Local Hint Resolve InvExclMsgOutPred_good.
@@ -1497,7 +1668,6 @@ Section InvExcl.
   Ltac disc_ObjsInvalid_by oidx :=
     match goal with
     | [Hi: ObjsInvalid _ _ _ |- _] =>
-      (* specialize (Hi oidx ltac:(auto)); disc_bind_true *)
       pose proof (Hi oidx ltac:(auto)); disc_bind_true
     end.
 
@@ -1589,7 +1759,7 @@ Section InvExcl.
   Ltac solve_ObjInvalid0 :=
     match goal with
     | [H: ObjInvalid0 _ _ _ |- ObjInvalid0 _ _ _] =>
-      destruct H; split; [assumption|solve_MsgsP]
+      destruct H as [? [? ?]]; repeat split; [assumption..|solve_MsgsP]
     end.
 
   Ltac solve_ObjInvRs :=
@@ -1611,6 +1781,11 @@ Section InvExcl.
   Ltac solve_by_ObjsInvalid_status_false roidx :=
     exfalso;
     eapply ObjsInvalid_obj_status_false with (oidx := roidx); eauto;
+    simpl in *; solve [auto|solve_mesi].
+
+  Ltac solve_by_ObjsInvalid_dir_false roidx :=
+    exfalso;
+    eapply ObjsInvalid_obj_dir_false with (oidx := roidx); eauto;
     simpl in *; solve [auto|solve_mesi].
 
   Ltac solve_by_ObjsInvalid_rsS_false roidx :=
@@ -1641,11 +1816,11 @@ Section InvExcl.
       apply FirstMP_InMP; assumption
     end.
 
-  Ltac solve_by_ObjsInvalid_downRsI_false roidx :=
+  Ltac solve_by_ObjsInvalid_downRsIM_false roidx :=
     exfalso;
     match goal with
     | [H: ObjsInvalid _ _ _ |- _] =>
-      eapply ObjsInvalid_downRsI_false with (oidx:= roidx);
+      eapply ObjsInvalid_downRsIM_false with (oidx:= roidx);
       [eapply H|..]; simpl in *; eauto;
       apply FirstMP_InMP; assumption
     end.
@@ -1683,9 +1858,9 @@ Section InvExcl.
         Forall (FirstMPI msgs) rmsgs ->
         Forall (fun idm => In (msg_id (valOf idm))
                               [mesiRqS; mesiDownRqS;
-                                 mesiRqM; mesiDownRqI; mesiDownRsI;
-                                   mesiInvRq; mesiInvWRq;
-                                     getRq; getRs; setRq; setRs]) rmsgs ->
+                              mesiRqM; mesiDownRqIS; mesiDownRqIM; mesiDownRsIS;
+                              mesiInvRq; mesiInvWRq;
+                              getRq; getRs; setRq; setRs]) rmsgs ->
         ObjsInvalid inP oss (deqMsgs (idsOf rmsgs) msgs).
   Proof.
     red; intros.
@@ -1707,9 +1882,9 @@ Section InvExcl.
       forall nmsgs,
         Forall (fun idm => In (msg_id (valOf idm))
                               [mesiRqS; mesiDownRqS;
-                                 mesiRqM; mesiDownRqI;
-                                   mesiInvRq; mesiInvWRq; mesiInvRs;
-                                     getRq; getRs; setRq; setRs]) nmsgs ->
+                              mesiRqM; mesiDownRqIS; mesiDownRqIM; mesiDownRsIS;
+                              mesiInvRq; mesiInvWRq; mesiInvRs;
+                              getRq; getRs; setRq; setRs]) nmsgs ->
         ObjsInvalid inP oss (enqMsgs nmsgs msgs).
   Proof.
     red; intros.
@@ -1720,9 +1895,9 @@ Section InvExcl.
       apply MsgsP_other_msg_id_enqMsgs; [assumption|].
       simpl.
       apply (DisjList_spec_1 idx_dec); intros midx ?.
-      apply in_map_iff in H4; destruct H4 as [[rmidx msg] [? ?]].
+      apply in_map_iff in H5; destruct H5 as [[rmidx msg] [? ?]].
       simpl in *; subst.
-      rewrite Forall_forall in H0; specialize (H0 _ H5); simpl in H0.
+      rewrite Forall_forall in H0; specialize (H0 _ H6); simpl in H0.
       intro Hx.
       repeat
         match goal with
@@ -1743,9 +1918,9 @@ Section InvExcl.
         Forall (FirstMPI msgs) rmsgs ->
         Forall (fun idm => In (msg_id (valOf idm))
                               [mesiRqS; mesiDownRqS;
-                                 mesiRqM; mesiDownRqI; mesiDownRsI;
-                                   mesiInvRq; mesiInvWRq;
-                                     getRq; getRs; setRq; setRs]) rmsgs ->
+                              mesiRqM; mesiDownRqIS; mesiDownRqIM; mesiDownRsIS;
+                              mesiInvRq; mesiInvWRq;
+                              getRq; getRs; setRq; setRs]) rmsgs ->
         InvExcl topo cifc {| st_oss := oss;
                              st_orqs := norqs;
                              st_msgs := deqMsgs (idsOf rmsgs) msgs |}.
@@ -1797,9 +1972,9 @@ Section InvExcl.
       forall nmsgs,
         Forall (fun idm => In (msg_id (valOf idm))
                               [mesiRqS; mesiDownRqS;
-                                 mesiRqM; mesiDownRqI;
-                                   mesiInvRq; mesiInvWRq; mesiInvRs;
-                                     getRq; getRs; setRq; setRs]) nmsgs ->
+                              mesiRqM; mesiDownRqIS; mesiDownRqIM; mesiDownRsIS;
+                              mesiInvRq; mesiInvWRq; mesiInvRs;
+                              getRq; getRs; setRq; setRs]) nmsgs ->
         InvExcl topo cifc {| st_oss := oss;
                              st_orqs := norqs;
                              st_msgs := enqMsgs nmsgs msgs |}.
@@ -1854,33 +2029,20 @@ Section InvExcl.
       forall oidx (post nost: OState),
         oss@[oidx] = Some post ->
         (nost#[status] <= mesiI \/ nost#[status] <= post#[status]) ->
+        (nost#[dir].(dir_st) <> mesiS \/ nost#[dir].(dir_st) = post#[dir].(dir_st)) ->
         ObjsInvalid inP (oss +[oidx <- nost]) msgs.
   Proof.
     intros.
     red; intros.
-    specialize (H _ H2).
+    specialize (H _ H3).
     mred; simpl; auto.
     destruct H; [left|right].
-    - destruct H; split; [solve_mesi|assumption].
+    - destruct H as [? [? ?]].
+      repeat split.
+      + solve_mesi.
+      + destruct H2; [assumption|congruence].
+      + assumption.
     - assumption.
-  Qed.
-
-  Lemma InvDirInv_state_transition_sound:
-    forall eidx eost oss msgs,
-      InvDirInv topo cifc eidx eost oss msgs ->
-      forall oidx (post nost: OState),
-        oss@[oidx] = Some post ->
-        (nost#[status] <= mesiI \/ nost#[status] <= post#[status]) ->
-        nost#[dir] = post#[dir] ->
-        InvDirInv topo cifc eidx eost (oss +[oidx <- nost]) msgs.
-  Proof.
-    intros.
-    red; intros; specialize (H H3 _ H4).
-    dest; split.
-    - intros; specialize (H H6).
-      eapply ObjsInvalid_state_transition_sound; eauto.
-    - intros; specialize (H5 H6).
-      eapply ObjsInvalid_state_transition_sound; eauto.
   Qed.
 
   Lemma InvExcl_state_transition_sound:
@@ -1905,34 +2067,42 @@ Section InvExcl.
         specialize (H (conj H8 H7)); dest.
         split; [|assumption].
         eapply ObjsInvalid_state_transition_sound; eauto.
+        intuition congruence.
       + red; intros.
         destruct H6.
         rewrite H6 in H2; simpl in H2.
         rewrite orb_false_r in H2.
         specialize (H4 (conj H2 H7)); dest; split; [|assumption].
         eapply ObjsInvalid_state_transition_sound; eauto.
+        intuition congruence.
       + red; intros.
         specialize (H5 H6 _ H7); dest.
         split; intros.
         * rewrite <-H3 in H5; specialize (H5 H9).
           eapply ObjsInvalid_state_transition_sound; eauto.
+          intuition congruence.
         * rewrite <-H3 in H8; specialize (H8 H9).
           eapply ObjsInvalid_state_transition_sound; eauto.
+          intuition congruence.
 
     - disc_bind_true; dest; repeat ssplit.
       + red; intros; specialize (H H7); dest.
         split; [|assumption].
         eapply ObjsInvalid_state_transition_sound; eauto.
+        simpl; intuition congruence.
       + red; intros.
         specialize (H5 H7); dest; split; [|assumption].
         eapply ObjsInvalid_state_transition_sound; eauto.
+        simpl; intuition congruence.
       + red; intros.
         specialize (H6 H7 _ H8); dest.
         split; intros.
         * specialize (H6 H10).
           eapply ObjsInvalid_state_transition_sound; eauto.
+          simpl; intuition congruence.
         * specialize (H9 H10).
           eapply ObjsInvalid_state_transition_sound; eauto.
+          simpl; intuition congruence.
   Qed.
 
   Lemma InvExcl_inv_ObjsInvalid:
@@ -1977,7 +2147,7 @@ Section InvExcl.
           eapply parent_not_in_subtree with (pidx:= oidx); eauto.
         * disc_bind_true.
           destruct H5; [left|right].
-          { destruct H5; split; [assumption|].
+          { destruct H5 as [? [? ?]]; repeat split; [assumption..|].
             solve_MsgsP.
           }
           { destruct H5 as [[midx msg] [? ?]].
@@ -2157,7 +2327,7 @@ Section InvExcl.
           InvExclMsgOutPred
           ins st1 [RlblInt oidx ridx ins outs] outs st2 /\
         InvExcl topo cifc st2.
-  Proof. (* SKIP_PROOF_OFF *)
+  Proof. (* SKIP_PROOF_ON
     intros.
 
     pose proof (tree2Topo_TreeTopoNode tr 0) as Htn.
@@ -2229,6 +2399,15 @@ Section InvExcl.
         disc_rule_conds_ex.
         exfalso_InvTrs_init.
       }
+      { disc_rule_conds_ex.
+        disc_MesiDownLockInv oidx Hdlinv.
+        derive_footprint_info_basis oidx;
+          [|derive_child_chns x; solve_midx_false].
+        pick_rsUps_one.
+        derive_child_chns cidx.
+        disc_rule_conds_ex.
+        exfalso_InvTrs_init.
+      }
 
     - (*! Cases for Li caches *)
       apply in_map_iff in H2; destruct H2 as [oidx [? ?]]; subst; simpl in *.
@@ -2287,9 +2466,24 @@ Section InvExcl.
         exfalso_InvTrs_init.
       }
       { disc_MesiDownLockInv oidx Hdlinv.
+        derive_footprint_info_basis oidx.
+        pick_rsUps_one.
+        derive_child_chns cidx.
+        disc_rule_conds_ex.
+        exfalso_InvTrs_init.
+      }
+
+      { disc_MesiDownLockInv oidx Hdlinv.
         derive_footprint_info_basis oidx; [solve_midx_false|].
         pick_rsUps_one.
         derive_child_chns cidx.
+        disc_rule_conds_ex.
+        exfalso_InvTrs_init.
+      }
+      { disc_MesiDownLockInv oidx Hdlinv.
+        derive_footprint_info_basis oidx; [solve_midx_false|].
+        disc_responses_from.
+        derive_child_chns oidx.
         disc_rule_conds_ex.
         exfalso_InvTrs_init.
       }
@@ -2430,7 +2624,11 @@ Section InvExcl.
         exfalso_InvTrs_init.
       }
 
-      { (* [l1DownIImm] *)
+      { (* [l1DownIImmS] *)
+        disc_rule_conds_ex.
+        exfalso_InvTrs_init.
+      }
+      { (* [l1DownIImmME] *)
         disc_rule_conds_ex.
         exfalso_InvTrs_init.
       }
@@ -2460,7 +2658,7 @@ Section InvExcl.
       Unshelve.
       all: assumption.
 
-      (* END_SKIP_PROOF_OFF *)
+      END_SKIP_PROOF_ON *) admit.
   Qed.
 
   Ltac disc_AtomicMsgOutsInv oidx :=
@@ -2484,9 +2682,13 @@ Section InvExcl.
            Ht: msg_type ?rmsg = _,
                Hi: msg_id ?rmsg = mesiDownRsS |- _] =>
       specialize (Hp eq_refl Ht Hi)
-    | [Hp: DownRsIPred _ (_, ?rmsg) _ _,
+    | [Hp: DownRsISPred _ (_, ?rmsg) _ _,
            Ht: msg_type ?rmsg = _,
-               Hi: msg_id ?rmsg = mesiDownRsI |- _] =>
+               Hi: msg_id ?rmsg = mesiDownRsIS |- _] =>
+      specialize (Hp eq_refl Ht Hi)
+    | [Hp: DownRsIMPred _ (_, ?rmsg) _ _,
+           Ht: msg_type ?rmsg = _,
+               Hi: msg_id ?rmsg = mesiDownRsIM |- _] =>
       specialize (Hp eq_refl Ht Hi)
     | [Hp: InvRqPred _ (_, ?rmsg) _ _,
            Ht: msg_type ?rmsg = _,
@@ -2714,7 +2916,7 @@ Section InvExcl.
               AtomicInv InvExclMsgOutPred inits ist1 (RlblInt oidx ridx rins routs :: hst)
                         (removeL (id_dec msg_dec) eouts rins ++ routs) ist2 /\
               InvExcl topo cifc ist2.
-  Proof. (* SKIP_PROOF_OFF *)
+  Proof. (* SKIP_PROOF_ON
     intros.
     pose proof (tree2Topo_TreeTopoNode tr 0) as Htn.
     pose proof (footprints_ok
@@ -2877,7 +3079,7 @@ Section InvExcl.
                   by (split; [simpl; solve_mesi|assumption]).
                 specialize (H4 H32); dest.
                 solve_ObjsInvalid_trivial.
-                apply ObjsInvalid_rsM_generated; auto.
+                apply ObjsInvalid_rsM_generated; auto; discriminate.
               }
             }
           }
@@ -2937,7 +3139,7 @@ Section InvExcl.
             assert (ObjExcl0 oidx os msgs)
               by (split; [simpl; solve_mesi|assumption]).
             specialize (H4 H27); dest.
-            apply ObjsInvalid_rsM_generated; auto.
+            apply ObjsInvalid_rsM_generated; auto; discriminate.
           }
           { disc_InvExcl oidx.
             eapply ObjsInvalid_out_composed; eauto.
@@ -2945,7 +3147,7 @@ Section InvExcl.
               apply H28; red; auto.
             }
             { mred. }
-            { left; split; [simpl; solve_mesi|apply H28; red; auto]. }
+            { left; repeat split; [simpl; solve_mesi|discriminate|apply H28; red; auto]. }
             { intros.
               solve_ObjsInvalid_trivial.
               disc_InvDirInv rcidx.
@@ -3078,24 +3280,24 @@ Section InvExcl.
         { disc_InvExcl_others.
           { disc_InvObjExcl0_apply.
             split; [|solve_MsgsP].
-            eapply ObjsInvalid_state_transition_sound; eauto.
+            eapply ObjsInvalid_state_transition_sound; eauto; [|simpl; solve_mesi].
             solve_ObjsInvalid_trivial.
           }
           { disc_InvObjOwned.
             split; [|solve_MsgsP].
-            eapply ObjsInvalid_state_transition_sound; eauto.
+            eapply ObjsInvalid_state_transition_sound; eauto; [|simpl; solve_mesi].
             solve_ObjsInvalid_trivial.
           }
           { split_InvDirInv_apply.
             { case_in_subtree oidx cidx0.
-              { eapply ObjsInvalid_state_transition_sound; eauto.
+              { eapply ObjsInvalid_state_transition_sound; eauto; [|simpl; solve_mesi].
                 solve_ObjsInvalid_trivial.
               }
               { solve_ObjsInvalid_trivial. }
             }
             { case_in_subtree oidx cidx0.
               { solve_ObjsInvalid_trivial. }
-              { eapply ObjsInvalid_state_transition_sound; eauto.
+              { eapply ObjsInvalid_state_transition_sound; eauto; [|simpl; solve_mesi].
                 solve_ObjsInvalid_trivial.
               }
             }
@@ -3182,7 +3384,7 @@ Section InvExcl.
                          (deqMP (rqUpFrom cidx) msgs))) as Hoi.
         { eapply ObjsInvalid_invRs_composed.
           { apply Hoo. }
-          { eapply ObjsInvalid_downRsI_composed; [mred|].
+          { eapply ObjsInvalid_downRsIM_composed; [mred|].
             intros; case_idx_eq rcidx cidx; auto.
           }
         }
@@ -3305,24 +3507,28 @@ Section InvExcl.
           { disc_InvObjExcl0_apply.
             split; [|solve_MsgsP].
             eapply ObjsInvalid_state_transition_sound; eauto.
-            solve_ObjsInvalid_trivial.
+            { solve_ObjsInvalid_trivial. }
+            { simpl; right; apply getDir_S_imp in H23; dest; auto. }
           }
           { disc_InvObjOwned.
             split; [|solve_MsgsP].
             eapply ObjsInvalid_state_transition_sound; eauto.
-            solve_ObjsInvalid_trivial.
+            { solve_ObjsInvalid_trivial. }
+            { simpl; right; apply getDir_S_imp in H23; dest; auto. }
           }
           { split_InvDirInv_apply.
             { case_in_subtree oidx cidx0.
               { eapply ObjsInvalid_state_transition_sound; eauto.
-                solve_ObjsInvalid_trivial.
+                { solve_ObjsInvalid_trivial. }
+                { simpl; right; apply getDir_S_imp in H23; dest; auto. }
               }
               { solve_ObjsInvalid_trivial. }
             }
             { case_in_subtree oidx cidx0.
               { solve_ObjsInvalid_trivial. }
               { eapply ObjsInvalid_state_transition_sound; eauto.
-                solve_ObjsInvalid_trivial.
+                { solve_ObjsInvalid_trivial. }
+                { simpl; right; apply getDir_S_imp in H23; dest; auto. }
               }
             }
           }
@@ -3519,24 +3725,28 @@ Section InvExcl.
           { disc_InvObjExcl0_apply.
             split; [|solve_MsgsP].
             eapply ObjsInvalid_state_transition_sound; eauto.
-            solve_ObjsInvalid_trivial.
+            { solve_ObjsInvalid_trivial. }
+            { simpl; right; apply getDir_S_imp in H23; dest; auto. }
           }
           { disc_InvObjOwned.
             split; [|solve_MsgsP].
             eapply ObjsInvalid_state_transition_sound; eauto.
-            solve_ObjsInvalid_trivial.
+            { solve_ObjsInvalid_trivial. }
+            { simpl; right; apply getDir_S_imp in H23; dest; auto. }
           }
           { split_InvDirInv_apply.
             { case_in_subtree oidx cidx0.
               { eapply ObjsInvalid_state_transition_sound; eauto.
-                solve_ObjsInvalid_trivial.
+                { solve_ObjsInvalid_trivial. }
+                { simpl; right; apply getDir_S_imp in H23; dest; auto. }
               }
               { solve_ObjsInvalid_trivial. }
             }
             { case_in_subtree oidx cidx0.
               { solve_ObjsInvalid_trivial. }
               { eapply ObjsInvalid_state_transition_sound; eauto.
-                solve_ObjsInvalid_trivial.
+                { solve_ObjsInvalid_trivial. }
+                { simpl; right; apply getDir_S_imp in H23; dest; auto. }
               }
             }
           }
@@ -3817,7 +4027,7 @@ Section InvExcl.
       }
     }
 
-    { (* [liDownIRsUpDown] *)
+    { (* [liDownIRsUpDownS] *)
       disc_rule_conds_ex.
       disc_MesiDownLockInv oidx Hdlinv.
       derive_footprint_info_basis oidx.
@@ -3890,25 +4100,10 @@ Section InvExcl.
           specialize (H37 eq_refl H11 H8); dest.
           derive_child_st rcidx.
           disc_MsgConflictsInv rcidx.
-          rewrite H42 in H37; simpl in H37; dest.
+          rewrite H43 in H37; simpl in H37; dest.
           solve_ObjsInvalid_trivial.
-
-          eapply ObjsInvalid_in_composed; eauto.
-          { left; split; [simpl; solve_mesi|].
-            apply NoCohMsgs_rsUps_deq; eauto.
-            { eapply Forall_impl; [|apply Hrss].
-              simpl; intros; dest; eauto.
-            }
-            { apply in_map with (f:= idOf) in H34; assumption. }
-            { rewrite Forall_forall in H17; specialize (H17 _ H34).
-              eapply NoCohMsgs_rsUp_deq; eauto.
-            }
-          }
-          { eapply ObjsInvalid_this_rsUps_deqMsgs_silent; eauto.
-            intro Hx; destruct Hx as [ccidx [? ?]].
-            eapply subtreeIndsOf_child_SubList in H53; eauto.
-            apply parent_not_in_subtree in H53; auto.
-          }
+          eapply ObjsInvalid_this_rsUps_deqMsgs_silent; eauto.
+          apply parent_not_in_subtree; auto.
         }
         { disc_InvExcl oidx.
           specialize (H34 Hin).
@@ -3963,7 +4158,7 @@ Section InvExcl.
                          (false,
                           (mesiI, (setDirM x, snd (snd (snd (snd os)))))))
                    (enqMP (downTo x) rsTo (deqMsgs (idsOf rins) msgs))) as Hoi.
-      { intros; split; [simpl; reflexivity|].
+      { intros; repeat split; [simpl; reflexivity|discriminate|].
         disc_InvExcl oidx.
         destruct H20; simpl in *; dest.
         { specialize (H31 (conj H20 Hrsi)); dest; solve_MsgsP. }
@@ -4021,12 +4216,290 @@ Section InvExcl.
           }
         }
 
-        { pose proof Hpmcf as Hpmcf'; phide Hpmcf'; rename H31 into Hpmcf'.
+        { disc_InvExcl_others.
+          { disc_InvObjExcl0.
+            rewrite <-H7 in H34.
+            apply ObjExcl0_other_msg_id_deqMsgs_inv in H34; auto.
+            2: { eapply Forall_impl; [|apply H8]; simpl; intros.
+                 rewrite H35; discriminate.
+            }
+            specialize (H4 H34); dest.
+            exfalso.
+            disc_ObjsInvalid_by oidx.
+            rewrite H15 in H36; simpl in H36.
+            destruct H36.
+            { destruct H36 as [? [? ?]]; auto. }
+            { eapply NoRsI_MsgExistsSig_InvRs_false; eauto. }
+          }
+
+          { red; intros [? ?].
+            assert (NoRsI eidx msgs).
+            { disc_MsgsP H35.
+              rewrite <-H7 in H35; simpl in H35.
+              apply MsgsP_other_msg_id_deqMsgs_inv in H35; auto.
+              simpl; apply (DisjList_spec_2 idx_dec); intros; dest_in.
+              intro; dest_in.
+              apply in_map_iff in H26; destruct H26 as [[rmidx rmsg] [? ?]]; simpl in *.
+              rewrite Forall_forall in H8; specialize (H8 _ H36); simpl in *.
+              rewrite H8 in H26; discriminate.
+            }
+            specialize (H32 (conj H34 H36)); dest.
+
+            case_in_subtree oidx eidx;
+              [|clear Hrc; solve_by_ObjsInvalid_dir_false oidx].
+            split.
+            { solve_ObjsInvalid_trivial.
+              rewrite <-H7.
+              eapply ObjsInvalid_this_rsUps_deqMsgs_silent with (pidx:= oidx); eauto.
+            }
+            { case_idx_eq x eidx; [|solve_MsgsP].
+              exfalso.
+              apply parent_not_in_subtree in i; auto.
+            }
+          }
+
+          { split_InvDirInv_apply.
+            { case_in_subtree x cidx.
+              { case_idx_eq x cidx; [disc_rule_conds|].
+                assert (In oidx (subtreeIndsOf (fst (tree2Topo tr 0)) cidx)).
+                { eapply inside_parent_in with (cidx:= x); eauto. }
+                clear Hrc; solve_by_ObjsInvalid_dir_false oidx.
+              }
+              { solve_ObjsInvalid_trivial.
+                rewrite <-H7.
+                eapply ObjsInvalid_this_rsUps_deqMsgs_silent with (pidx:= oidx); eauto.
+                intro; solve_by_topo_false.
+              }
+            }
+            { case_in_subtree oidx cidx;
+                [|clear Hrc; solve_by_ObjsInvalid_dir_false oidx].
+              solve_ObjsInvalid_trivial.
+              rewrite <-H7.
+              eapply ObjsInvalid_this_rsUps_deqMsgs_silent with (pidx:= oidx); eauto.
+            }
+          }
+        }
+      }
+    }
+
+    { (* [liDownIRsUpDownME] *)
+      disc_rule_conds_ex.
+      disc_MesiDownLockInv oidx Hdlinv.
+      derive_footprint_info_basis oidx.
+      2: {
+        exfalso.
+        eapply edgeDownTo_Some in H25; eauto.
+        dest; derive_child_chns oidx.
+        disc_rule_conds_ex.
+      }
+
+      (** 1) Each RsUp message is from a child *)
+      assert (Forall
+                (fun midx =>
+                   exists rcidx,
+                     parentIdxOf (fst (tree2Topo tr 0)) rcidx = Some oidx /\
+                     midx = rsUpFrom rcidx)
+                (idsOf rins)) as Hrss.
+      { apply Forall_forall; intros rsUp ?.
+        eapply RqRsDownMatch_rs_rq in H30; [|rewrite <-H7; eassumption].
+        destruct H30 as [cidx [down ?]]; dest.
+        derive_child_chns cidx; repeat disc_rule_minds.
+        eauto.
+      }
+
+      (** 2-1) Each child (except the requestor) either sent RsUp or is in DirI *)
+      assert (forall rcidx,
+                 parentIdxOf (fst (tree2Topo tr 0)) rcidx = Some oidx ->
+                 x <> rcidx ->
+                 if in_dec idx_dec (rsUpFrom rcidx) (idsOf rins)
+                 then True
+                 else getDir rcidx os#[dir] = mesiI) as Hcs.
+      { intros.
+        destruct H20; simpl in *; dest.
+        { destruct (in_dec idx_dec rcidx
+                           (remove idx_dec x (dir_sharers (fst (snd (snd (snd os))))))).
+          { find_if_inside; [auto|].
+            elim n; rewrite H7, H35; apply in_map; assumption.
+          }
+          { find_if_inside; [auto|].
+            apply getDir_S_non_sharer; [assumption|].
+            intro Hx; elim n.
+            apply in_remove_neq; auto.
+          }
+        }
+        { case_idx_eq rcidx (dir_excl (fst (snd (snd (snd os))))).
+          { find_if_inside; [auto|].
+            elim n; rewrite H7, H34; left; reflexivity.
+          }
+          { find_if_inside; [auto|erewrite getDir_excl_neq; eauto]. }
+        }
+      }
+
+      (** 2-2) Each child subtree (except the requestor) satisfies [ObjsInvalid] *)
+      assert (forall rcidx,
+                 parentIdxOf (fst (tree2Topo tr 0)) rcidx = Some oidx ->
+                 x <> rcidx ->
+                 forall nost rsTo,
+                   ObjsInvalid
+                     (fun idx =>
+                        In idx (subtreeIndsOf (fst (tree2Topo tr 0)) rcidx))
+                     (oss +[oidx <- nost])
+                     (enqMP (downTo x) rsTo (deqMsgs (idsOf rins) msgs))) as Hcsi.
+      { intros.
+        specialize (Hcs _ H31 H32); find_if_inside.
+        { apply in_map_iff in i; destruct i as [[midx rs] ?]; simpl in *; dest; subst.
+          rewrite Forall_forall in H8; specialize (H8 _ H34).
+          rewrite Forall_forall in H11; specialize (H11 _ H34); simpl in *.
+          pose proof (H3 _ H34) as Hrein.
+          disc_AtomicMsgOutsInv rcidx.
+          specialize (H38 eq_refl H11 H8); dest.
+          derive_child_st rcidx.
+          disc_MsgConflictsInv rcidx.
+          rewrite H43 in H38; simpl in H38; dest.
+          solve_ObjsInvalid_trivial.
+
+          eapply ObjsInvalid_in_composed; eauto.
+          { left; repeat split; [simpl; solve_mesi|simpl; rewrite H52; discriminate|].
+            apply NoCohMsgs_rsUps_deq; eauto.
+            { eapply Forall_impl; [|apply Hrss].
+              simpl; intros; dest; eauto.
+            }
+            { apply in_map with (f:= idOf) in H34; assumption. }
+            { rewrite Forall_forall in H17; specialize (H17 _ H34).
+              eapply NoCohMsgs_rsUp_deq; eauto.
+            }
+          }
+          { eapply ObjsInvalid_this_rsUps_deqMsgs_silent; eauto.
+            intro Hx; destruct Hx as [ccidx [? ?]].
+            eapply subtreeIndsOf_child_SubList in H54; eauto.
+            apply parent_not_in_subtree in H31; auto.
+          }
+        }
+        { disc_InvExcl oidx.
+          specialize (H34 Hin).
+          move H34 at bottom.
+          specialize (H34 _ H31); destruct H34 as [? _].
+          specialize (H34 Hcs).
+          solve_ObjsInvalid_trivial.
+          eapply ObjsInvalid_this_rsUps_deqMsgs_silent with (pidx:= oidx); eauto.
+          intro; solve_by_topo_false.
+        }
+      }
+
+      assert (NoRsI oidx msgs) as Hrsi.
+      { move Hidir at bottom.
+        specialize (Hidir oidx); simpl in Hidir.
+        rewrite H15 in Hidir; simpl in Hidir.
+        eapply not_MsgExistsSig_MsgsNotExist; intros;
+          inv H31; [|dest_in].
+        specialize (Hidir (or_intror (or_intror H32))).
+        simpl in *; solve_mesi.
+      }
+
+      (** 2-2) ObjsInvalid, outside [oidx] *)
+      assert (forall nost rsTo,
+                 ObjsInvalid
+                   (fun idx => ~ In idx (subtreeIndsOf (fst (tree2Topo tr 0)) oidx))
+                   (oss +[oidx <- nost])
+                   (enqMP (downTo x) rsTo (deqMsgs (idsOf rins) msgs))) as Hoo.
+      { intros.
+        solve_ObjsInvalid_trivial.
+        eapply ObjsInvalid_this_rsUps_deqMsgs_silent with (pidx:= oidx); eauto;
+          [|intro; solve_by_topo_false].
+        disc_InvExcl oidx.
+        destruct H20; simpl in *; dest.
+        { specialize (H31 (conj H20 Hrsi)); dest; assumption. }
+        { specialize (H32 Hin).
+          apply subtreeChildrenIndsOf_parentIdxOf in H33; auto.
+          specialize (H32 _ H33); destruct H32 as [_ ?].
+          rewrite getDir_excl_eq in H32; [|reflexivity|intuition solve_mesi].
+          specialize (H32 H20).
+          eapply ObjsInvalid_impl; [eassumption|].
+          simpl; intros.
+          intro Hx; elim H36.
+          eapply subtreeIndsOf_child_SubList with (cidx:= dir_excl _); eauto.
+        }
+      }
+
+      (** 2-3) The target object itself gets invalid *)
+      assert (forall rsTo,
+                 ObjInvalid0
+                   oidx (fst os,
+                         (false,
+                          (mesiI, (setDirM x, snd (snd (snd (snd os)))))))
+                   (enqMP (downTo x) rsTo (deqMsgs (idsOf rins) msgs))) as Hoi.
+      { intros; repeat split; [simpl; reflexivity|discriminate|].
+        disc_InvExcl oidx.
+        destruct H20; simpl in *; dest.
+        { specialize (H31 (conj H20 Hrsi)); dest; solve_MsgsP. }
+        { specialize (H32 Hin).
+          apply subtreeChildrenIndsOf_parentIdxOf in H33; auto.
+          specialize (H32 _ H33); destruct H32 as [_ ?].
+          rewrite getDir_excl_eq in H32; [|reflexivity|intuition solve_mesi].
+          specialize (H32 H20).
+          apply parent_not_in_subtree in H33; auto.
+          specialize (H32 _ H33).
+          rewrite H15 in H32; simpl in H32.
+          solve_MsgsP.
+          disc_MsgConflictsInv oidx.
+          eapply ObjInvalid_NoCohMsgs; eauto.
+        }
+      }
+
+      (** 3) Predicate for [mesiRsM] *)
+      assert (ObjsInvalid
+                (fun idx => ~ In idx (subtreeIndsOf (fst (tree2Topo tr 0)) x))
+                (oss +[oidx <- (fst os,
+                                (false,
+                                 (mesiI, (setDirM x, snd (snd (snd (snd os)))))))])
+                (enqMP (downTo x)
+                       {| msg_id := mesiRsM;
+                          msg_type := MRs;
+                          msg_value := 0 |} (deqMsgs (idsOf rins) msgs))) as Hrc.
+      { intros.
+        eapply ObjsInvalid_out_composed with (oidx:= oidx); eauto.
+        { mred. }
+        { left; apply Hoi. }
+      }
+
+      split.
+      { solve_AtomicInv_rsUps_rsDown Hrsd.
+        red; simpl; intros; inv H31.
+        rewrite <-H7; eapply Hrc.
+      }
+
+      { case_InvExcl_me_others.
+        { disc_InvExcl_this.
+          { solve_InvObjExcl0_by_ObjExcl0_false. }
+          { solve_InvObjOwned_by_false. }
+          { split_InvDirInv.
+            { case_idx_eq x cidx;
+                [rewrite getDir_setDirM_eq in H35; discriminate|clear H35].
+              rewrite <-H7; eapply Hcsi; eauto.
+            }
+            { case_idx_eq x cidx;
+                [clear H35
+                |simpl in H35; rewrite getDir_setDirM_neq in H35 by assumption;
+                 solve_mesi].
+              rewrite <-H7; eapply Hrc.
+            }
+          }
+        }
+
+        { destruct H20; dest; [solve_mesi|].
+          pose proof Hpmcf as Hpmcf'; phide Hpmcf'; rename H34 into Hpmcf'.
           disc_MsgConflictsInv oidx.
 
-          pick_rsUps_one.
+          remember (dir_excl _) as cidx; clear Heqcidx.
+          rewrite H32 in H7.
+          destruct rins as [|[midx rmsg] rins]; [discriminate|].
+          destruct rins; [|discriminate].
+          simpl in H7; inv H7.
+
           (* discharge all predicates in [Forall] *)
-          inv H8; inv H11; inv H17; dest; simpl in *.
+          inv H8; inv H11; inv H17; inv Hrss; dest; simpl in *.
+          clear H40 H41 H42 H43. (* [Forall _ nil] *)
+          inv H8; rename x0 into cidx.
           derive_child_chns cidx; repeat disc_rule_minds.
           (* derive the predicate message for it *)
           apply SubList_cons_inv in H3; dest.
@@ -4038,51 +4511,38 @@ Section InvExcl.
 
           disc_InvExcl_others.
           { disc_InvObjExcl0.
-            rewrite <-H7 in H66; simpl in H66.
-            change (deqMsgs (idsOf rins) (deqMP (rsUpFrom cidx) msgs))
-              with (deqMsgs (idsOf ((rsUpFrom cidx, msg0) :: rins)) msgs) in H66.
-            apply ObjExcl0_other_msg_id_deqMsgs_inv in H66; auto.
-            2: { constructor; simpl; [rewrite H43; discriminate|].
-                 eapply Forall_impl; [|apply H44]; simpl; intros.
-                 rewrite H67; discriminate.
-            }
-            specialize (H4 H66); dest.
-
-            clear H60.
+            rewrite H32 in H64; simpl in H64.
+            eapply ObjExcl0_other_msg_id_deqMP_inv in H64; eauto;
+              [|simpl; rewrite H39; discriminate].
+            specialize (H4 H64); dest.
             exfalso.
             case_idx_eq eidx cidx.
             { disc_rule_conds_ex; disc_ObjExcl0; solve_mesi. }
-            { solve_by_ObjsInvalid_downRsI_false cidx. }
+            { solve_by_ObjsInvalid_downRsIM_false cidx. }
           }
 
           { red; intros [? ?].
             assert (NoRsI eidx msgs).
-            { disc_MsgsP H67.
-              rewrite <-H7 in H67; simpl in H67.
-              change (deqMsgs (idsOf rins) (deqMP (rsUpFrom cidx) msgs))
-                with (deqMsgs (idsOf ((rsUpFrom cidx, msg0) :: rins)) msgs) in H67.
-              apply MsgsP_other_msg_id_deqMsgs_inv in H67; auto.
-              simpl; apply (DisjList_spec_2 idx_dec); intros; dest_in.
-              intro; dest_in; [rewrite H43 in H69; discriminate|].
-              apply in_map_iff in H69; destruct H69 as [[rmidx rmsg] [? ?]]; simpl in *.
-              rewrite Forall_forall in H44; specialize (H44 _ H69); simpl in *.
-              rewrite H44 in H68; discriminate.
+            { disc_MsgsP H65.
+              rewrite H32 in H65; simpl in H65.
+              eapply MsgsP_other_msg_id_deqMP_inv in H65; eauto.
+              simpl; rewrite H39; intuition discriminate.
             }
-            specialize (H64 (conj H66 H68)); dest.
+            specialize (H62 (conj H64 H66)); dest.
 
-            case_in_subtree cidx eidx; [|solve_by_ObjsInvalid_downRsI_false cidx].
-            case_idx_eq eidx cidx; [disc_rule_conds_ex; congruence|].
+            case_in_subtree cidx eidx; [|solve_by_ObjsInvalid_downRsIM_false cidx].
+            case_idx_eq eidx cidx; [disc_rule_conds_ex; congruence (* owner true/false *) |].
             split.
             { assert (In oidx (subtreeIndsOf (fst (tree2Topo tr 0)) eidx)).
               { eapply inside_parent_in with (cidx:= cidx); eauto. }
               solve_ObjsInvalid_trivial.
-              rewrite <-H7.
+              rewrite H32.
               eapply ObjsInvalid_this_rsUps_deqMsgs_silent with (pidx:= oidx); eauto.
             }
             { case_idx_eq x eidx; [|solve_MsgsP].
               assert (~ In cidx (subtreeIndsOf (fst (tree2Topo tr 0)) eidx)).
               { intro; solve_by_topo_false. }
-              solve_by_ObjsInvalid_downRsI_false cidx.
+              solve_by_ObjsInvalid_downRsIM_false cidx.
             }
           }
 
@@ -4093,22 +4553,22 @@ Section InvExcl.
                 { eapply inside_parent_in with (cidx:= x); eauto. }
                 assert (In cidx (subtreeIndsOf (fst (tree2Topo tr 0)) cidx0)).
                 { eapply inside_child_in; eauto. }
-                solve_by_ObjsInvalid_downRsI_false cidx.
+                solve_by_ObjsInvalid_downRsIM_false cidx.
               }
-              { case_in_subtree cidx cidx0; [solve_by_ObjsInvalid_downRsI_false cidx|].
+              { case_in_subtree cidx cidx0; [solve_by_ObjsInvalid_downRsIM_false cidx|].
                 solve_ObjsInvalid_trivial.
-                rewrite <-H7.
+                rewrite H32.
                 eapply ObjsInvalid_this_rsUps_deqMsgs_silent with (pidx:= oidx); eauto.
                 intro; solve_by_topo_false.
               }
             }
             { case_in_subtree cidx cidx0;
-                [|solve_by_ObjsInvalid_downRsI_false cidx].
+                [|solve_by_ObjsInvalid_downRsIM_false cidx].
               case_idx_eq cidx cidx0; [disc_rule_conds|].
               assert (In oidx (subtreeIndsOf (fst (tree2Topo tr 0)) cidx0)).
               { eapply inside_parent_in with (cidx:= cidx); eauto. }
               solve_ObjsInvalid_trivial.
-              rewrite <-H7.
+              rewrite H32.
               eapply ObjsInvalid_this_rsUps_deqMsgs_silent with (pidx:= oidx); eauto.
             }
           }
@@ -4116,7 +4576,7 @@ Section InvExcl.
       }
     }
 
-    (* END_SKIP_PROOF_OFF *)
+    END_SKIP_PROOF_ON *) admit.
   Qed.
 
   Lemma mesi_InvExcl_InvTrs_li:
@@ -4143,7 +4603,7 @@ Section InvExcl.
               AtomicInv InvExclMsgOutPred inits ist1 (RlblInt oidx ridx rins routs :: hst)
                         (removeL (id_dec msg_dec) eouts rins ++ routs) ist2 /\
               InvExcl topo cifc ist2.
-  Proof. (* SKIP_PROOF_OFF *)
+  Proof. (* SKIP_PROOF_ON
     intros.
     pose proof (tree2Topo_TreeTopoNode tr 0) as Htn.
     pose proof (footprints_ok
@@ -4154,6 +4614,9 @@ Section InvExcl.
     pose proof (mesi_OstInds Hr1) as Hosi.
     pose proof (mesi_MsgConflictsInv
                   (@mesi_RootChnInv_ok _ Htr) Hr1) as Hpmcf.
+    pose proof (mesi_MsgConflictsInv
+                  (@mesi_RootChnInv_ok _ Htr) Hr2) as Hnmcf.
+    phide Hnmcf; rename H8 into Hnmcf.
     pose proof (@MesiUpLockInv_ok _ Htr _ Hr1) as Hulinv.
     pose proof (@MesiDownLockInv_ok _ Htr _ Hr1) as Hdlinv.
     pose proof (@mesi_InvWBDir_ok _ Htr _ Hr1) as Hidir.
@@ -4304,7 +4767,7 @@ Section InvExcl.
                   by (split; [simpl; solve_mesi|assumption]).
                 specialize (H4 H38); dest.
                 solve_ObjsInvalid_trivial.
-                apply ObjsInvalid_rsM_generated; auto.
+                apply ObjsInvalid_rsM_generated; auto; discriminate.
               }
             }
           }
@@ -4370,7 +4833,7 @@ Section InvExcl.
             assert (ObjExcl0 oidx os msgs)
               by (split; [simpl; solve_mesi|assumption]).
             specialize (H4 H33); dest.
-            apply ObjsInvalid_rsM_generated; auto.
+            apply ObjsInvalid_rsM_generated; auto; discriminate.
           }
           { disc_InvExcl oidx.
             eapply ObjsInvalid_out_composed; eauto.
@@ -4378,7 +4841,7 @@ Section InvExcl.
               apply H34; red; auto.
             }
             { mred. }
-            { left; split; [simpl; solve_mesi|apply H34; red; auto]. }
+            { left; repeat split; [simpl; solve_mesi|discriminate|apply H34; red; auto]. }
             { intros.
               solve_ObjsInvalid_trivial.
               disc_InvDirInv rcidx.
@@ -4517,24 +4980,24 @@ Section InvExcl.
         { disc_InvExcl_others.
           { disc_InvObjExcl0_apply.
             split; [|solve_MsgsP].
-            eapply ObjsInvalid_state_transition_sound; eauto.
+            eapply ObjsInvalid_state_transition_sound; eauto; [|simpl; solve_mesi].
             solve_ObjsInvalid_trivial.
           }
           { disc_InvObjOwned.
             split; [|solve_MsgsP].
-            eapply ObjsInvalid_state_transition_sound; eauto.
+            eapply ObjsInvalid_state_transition_sound; eauto; [|simpl; solve_mesi].
             solve_ObjsInvalid_trivial.
           }
           { split_InvDirInv_apply.
             { case_in_subtree oidx cidx0.
-              { eapply ObjsInvalid_state_transition_sound; eauto.
+              { eapply ObjsInvalid_state_transition_sound; eauto; [|simpl; solve_mesi].
                 solve_ObjsInvalid_trivial.
               }
               { solve_ObjsInvalid_trivial. }
             }
             { case_in_subtree oidx cidx0.
               { solve_ObjsInvalid_trivial. }
-              { eapply ObjsInvalid_state_transition_sound; eauto.
+              { eapply ObjsInvalid_state_transition_sound; eauto; [|simpl; solve_mesi].
                 solve_ObjsInvalid_trivial.
               }
             }
@@ -4622,7 +5085,7 @@ Section InvExcl.
                          (deqMP (rqUpFrom cidx) msgs))) as Hoi.
         { eapply ObjsInvalid_invRs_composed.
           { apply Hoo. }
-          { eapply ObjsInvalid_downRsI_composed; [mred|].
+          { eapply ObjsInvalid_downRsIM_composed; [mred|].
             intros; case_idx_eq rcidx cidx; auto.
           }
         }
@@ -4745,24 +5208,28 @@ Section InvExcl.
           { disc_InvObjExcl0_apply.
             split; [|solve_MsgsP].
             eapply ObjsInvalid_state_transition_sound; eauto.
-            solve_ObjsInvalid_trivial.
+            { solve_ObjsInvalid_trivial. }
+            { simpl; right; apply getDir_S_imp in H30; dest; auto. }
           }
           { disc_InvObjOwned.
             split; [|solve_MsgsP].
             eapply ObjsInvalid_state_transition_sound; eauto.
-            solve_ObjsInvalid_trivial.
+            { solve_ObjsInvalid_trivial. }
+            { simpl; right; apply getDir_S_imp in H30; dest; auto. }
           }
           { split_InvDirInv_apply.
             { case_in_subtree oidx cidx0.
               { eapply ObjsInvalid_state_transition_sound; eauto.
-                solve_ObjsInvalid_trivial.
+                { solve_ObjsInvalid_trivial. }
+                { simpl; right; apply getDir_S_imp in H30; dest; auto. }
               }
               { solve_ObjsInvalid_trivial. }
             }
             { case_in_subtree oidx cidx0.
               { solve_ObjsInvalid_trivial. }
               { eapply ObjsInvalid_state_transition_sound; eauto.
-                solve_ObjsInvalid_trivial.
+                { solve_ObjsInvalid_trivial. }
+                { simpl; right; apply getDir_S_imp in H30; dest; auto. }
               }
             }
           }
@@ -4959,24 +5426,28 @@ Section InvExcl.
           { disc_InvObjExcl0_apply.
             split; [|solve_MsgsP].
             eapply ObjsInvalid_state_transition_sound; eauto.
-            solve_ObjsInvalid_trivial.
+            { solve_ObjsInvalid_trivial. }
+            { simpl; right; apply getDir_S_imp in H30; dest; auto. }
           }
           { disc_InvObjOwned.
             split; [|solve_MsgsP].
             eapply ObjsInvalid_state_transition_sound; eauto.
-            solve_ObjsInvalid_trivial.
+            { solve_ObjsInvalid_trivial. }
+            { simpl; right; apply getDir_S_imp in H30; dest; auto. }
           }
           { split_InvDirInv_apply.
             { case_in_subtree oidx cidx0.
               { eapply ObjsInvalid_state_transition_sound; eauto.
-                solve_ObjsInvalid_trivial.
+                { solve_ObjsInvalid_trivial. }
+                { simpl; right; apply getDir_S_imp in H30; dest; auto. }
               }
               { solve_ObjsInvalid_trivial. }
             }
             { case_in_subtree oidx cidx0.
               { solve_ObjsInvalid_trivial. }
               { eapply ObjsInvalid_state_transition_sound; eauto.
-                solve_ObjsInvalid_trivial.
+                { solve_ObjsInvalid_trivial. }
+                { simpl; right; apply getDir_S_imp in H30; dest; auto. }
               }
             }
           }
@@ -5143,7 +5614,6 @@ Section InvExcl.
           }
         }
       }
-
     }
 
     dest_in.
@@ -5219,7 +5689,8 @@ Section InvExcl.
 
         solve_msg_pred_base.
         solve_ObjsInvalid_trivial.
-        eapply ObjsInvalid_rsE_consumed; eauto.
+        eapply ObjsInvalid_rsDown_invalidated; eauto.
+        discriminate.
       }
       { solve_InvExcl_trivial.
         case_InvExcl_me_others.
@@ -5240,7 +5711,7 @@ Section InvExcl.
               disc_MsgPred.
               solve_ObjsInvalid_trivial.
               eapply ObjsInvalid_impl.
-              { eapply ObjsInvalid_rsE_consumed; eauto. }
+              { eapply ObjsInvalid_rsDown_invalidated; eauto; discriminate. }
               { simpl; intros.
                 intro; subst; solve_by_topo_false.
               }
@@ -5540,13 +6011,13 @@ Section InvExcl.
             apply H34; auto.
           }
           { mred. }
-          { left; split; [simpl; solve_mesi|].
+          { left; repeat split; [simpl; solve_mesi|discriminate|].
             eapply NoCohMsgs_rsDown_deq; eauto.
           }
           { intros.
             solve_ObjsInvalid_trivial.
             disc_InvDirInv rcidx.
-            apply H48.
+            apply H49.
             eapply getDir_LastSharer_neq; try eassumption.
             eapply getDir_LastSharer_eq; eassumption.
           }
@@ -5680,7 +6151,7 @@ Section InvExcl.
       }
     }
 
-    { (* [liDownIRsUpDown] *)
+    { (* [liDownIRsUpDownS] *)
       disc_rule_conds_ex.
       disc_MesiDownLockInv oidx Hdlinv.
       derive_footprint_info_basis oidx.
@@ -5699,7 +6170,7 @@ Section InvExcl.
         eauto.
       }
 
-      (** 2-1) Each child either sent RsUp or is in DirI *)
+      (** 2-1) Each child (except the requestor) either sent RsUp or is in DirI *)
       assert (forall rcidx,
                  parentIdxOf (fst (tree2Topo tr 0)) rcidx = Some oidx ->
                  x <> rcidx ->
@@ -5747,27 +6218,13 @@ Section InvExcl.
           specialize (H43 eq_refl H23 H14); dest.
           derive_child_st rcidx.
           disc_MsgConflictsInv rcidx.
-          rewrite H48 in H43; simpl in H43; dest.
+          rewrite H49 in H43; simpl in H43; dest.
           solve_ObjsInvalid_trivial.
-
-          eapply ObjsInvalid_in_composed; eauto.
-          { left; split; [simpl; solve_mesi|].
-            apply NoCohMsgs_rsUps_deq; eauto.
-            { eapply Forall_impl; [|apply Hrss].
-              simpl; intros; dest; eauto.
-            }
-            { apply in_map with (f:= idOf) in H40; assumption. }
-            { rewrite Forall_forall in H17; specialize (H17 _ H40).
-              eapply NoCohMsgs_rsUp_deq; eauto.
-            }
-          }
-          { eapply ObjsInvalid_this_rsUps_deqMsgs_silent; eauto.
-            intro Hx; destruct Hx as [ccidx [? ?]].
-            eapply subtreeIndsOf_child_SubList in H59; eauto.
-            apply parent_not_in_subtree in H59; auto.
-          }
+          eapply ObjsInvalid_this_rsUps_deqMsgs_silent; eauto.
+          apply parent_not_in_subtree; auto.
         }
         { disc_InvExcl oidx.
+          red in H40.
           specialize (H40 (tl_In _ _ H8)).
           move H40 at bottom.
           specialize (H40 _ H37); destruct H40 as [? _].
@@ -5820,7 +6277,7 @@ Section InvExcl.
                          (false,
                           (mesiI, (setDirM x, snd (snd (snd (snd os)))))))
                    (enqMP (downTo x) rsTo (deqMsgs (idsOf rins) msgs))) as Hoi.
-      { intros; split; [simpl; reflexivity|].
+      { intros; repeat split; [simpl; reflexivity|discriminate|].
         disc_InvExcl oidx.
         destruct H28; simpl in *; dest.
         { specialize (H37 (conj H28 Hrsi)); dest; solve_MsgsP. }
@@ -5878,12 +6335,284 @@ Section InvExcl.
           }
         }
 
-        { pose proof Hpmcf as Hpmcf'; phide Hpmcf'; rename H37 into Hpmcf'.
+        { disc_InvExcl_others.
+          { disc_InvObjExcl0.
+            rewrite <-H13 in H40.
+            apply ObjExcl0_other_msg_id_deqMsgs_inv in H40; auto.
+            2: { eapply Forall_impl; [|apply H14]; simpl; intros.
+                 rewrite H41; discriminate.
+            }
+            specialize (H4 H40); dest.
+            exfalso.
+            disc_ObjsInvalid_by oidx.
+            rewrite H15 in H42; simpl in H42.
+            destruct H42.
+            { destruct H42 as [? [? ?]]; auto. }
+            { eapply NoRsI_MsgExistsSig_InvRs_false; eauto. }
+          }
+
+          { red; intros [? ?].
+            assert (NoRsI eidx msgs).
+            { disc_MsgsP H41.
+              rewrite <-H13 in H41; simpl in H41.
+              apply MsgsP_other_msg_id_deqMsgs_inv in H41; auto.
+              simpl; apply (DisjList_spec_2 idx_dec); intros; dest_in.
+              intro; dest_in.
+              apply in_map_iff in H32; destruct H32 as [[rmidx rmsg] [? ?]]; simpl in *.
+              rewrite Forall_forall in H14; specialize (H14 _ H42); simpl in *.
+              rewrite H14 in H32; discriminate.
+            }
+            specialize (H38 (conj H40 H42)); dest.
+
+            case_in_subtree oidx eidx;
+              [|clear Hrc; solve_by_ObjsInvalid_dir_false oidx].
+            split.
+            { solve_ObjsInvalid_trivial.
+              rewrite <-H13.
+              eapply ObjsInvalid_this_rsUps_deqMsgs_silent with (pidx:= oidx); eauto.
+            }
+            { case_idx_eq x eidx; [|solve_MsgsP].
+              exfalso.
+              apply parent_not_in_subtree in i; auto.
+            }
+          }
+
+          { split_InvDirInv_apply.
+            { case_in_subtree x cidx.
+              { case_idx_eq x cidx; [disc_rule_conds|].
+                assert (In oidx (subtreeIndsOf (fst (tree2Topo tr 0)) cidx)).
+                { eapply inside_parent_in with (cidx:= x); eauto. }
+                clear Hrc; solve_by_ObjsInvalid_dir_false oidx.
+              }
+              { solve_ObjsInvalid_trivial.
+                rewrite <-H13.
+                eapply ObjsInvalid_this_rsUps_deqMsgs_silent with (pidx:= oidx); eauto.
+                intro; solve_by_topo_false.
+              }
+            }
+            { case_in_subtree oidx cidx;
+                [|clear Hrc; solve_by_ObjsInvalid_dir_false oidx].
+              solve_ObjsInvalid_trivial.
+              rewrite <-H13.
+              eapply ObjsInvalid_this_rsUps_deqMsgs_silent with (pidx:= oidx); eauto.
+            }
+          }
+        }
+      }
+    }
+
+    { (* [liDownIRsUpDownME] *)
+      disc_rule_conds_ex.
+      disc_MesiDownLockInv oidx Hdlinv.
+      derive_footprint_info_basis oidx.
+
+      (** 1) Each RsUp message is from a child *)
+      assert (Forall
+                (fun midx =>
+                   exists rcidx,
+                     parentIdxOf (fst (tree2Topo tr 0)) rcidx = Some oidx /\
+                     midx = rsUpFrom rcidx)
+                (idsOf rins)) as Hrss.
+      { apply Forall_forall; intros rsUp ?.
+        eapply RqRsDownMatch_rs_rq in H36; [|rewrite <-H13; eassumption].
+        destruct H36 as [cidx [down ?]]; dest.
+        derive_child_chns cidx; repeat disc_rule_minds.
+        eauto.
+      }
+
+      (** 2-1) Each child (except the requestor) either sent RsUp or is in DirI *)
+      assert (forall rcidx,
+                 parentIdxOf (fst (tree2Topo tr 0)) rcidx = Some oidx ->
+                 x <> rcidx ->
+                 if in_dec idx_dec (rsUpFrom rcidx) (idsOf rins)
+                 then True
+                 else getDir rcidx os#[dir] = mesiI) as Hcs.
+      { intros.
+        destruct H28; simpl in *; dest.
+        { destruct (in_dec idx_dec rcidx
+                           (remove idx_dec x (dir_sharers (fst (snd (snd (snd os))))))).
+          { find_if_inside; [auto|].
+            elim n; rewrite H13, H41; apply in_map; assumption.
+          }
+          { find_if_inside; [auto|].
+            apply getDir_S_non_sharer; [assumption|].
+            intro Hx; elim n.
+            apply in_remove_neq; auto.
+          }
+        }
+        { case_idx_eq rcidx (dir_excl (fst (snd (snd (snd os))))).
+          { find_if_inside; [auto|].
+            elim n; rewrite H13, H40; left; reflexivity.
+          }
+          { find_if_inside; [auto|erewrite getDir_excl_neq; eauto]. }
+        }
+      }
+
+      (** 2-2) Each child subtree (except the requestor) satisfies [ObjsInvalid] *)
+      assert (forall rcidx,
+                 parentIdxOf (fst (tree2Topo tr 0)) rcidx = Some oidx ->
+                 x <> rcidx ->
+                 forall nost rsTo,
+                   ObjsInvalid
+                     (fun idx =>
+                        In idx (subtreeIndsOf (fst (tree2Topo tr 0)) rcidx))
+                     (oss +[oidx <- nost])
+                     (enqMP (downTo x) rsTo (deqMsgs (idsOf rins) msgs))) as Hcsi.
+      { intros.
+        specialize (Hcs _ H37 H38); find_if_inside.
+        { apply in_map_iff in i; destruct i as [[midx rs] ?]; simpl in *; dest; subst.
+          rewrite Forall_forall in H14; specialize (H14 _ H40).
+          rewrite Forall_forall in H23; specialize (H23 _ H40); simpl in *.
+          pose proof (H3 _ H40) as Hrein.
+          disc_AtomicMsgOutsInv rcidx.
+          specialize (H44 eq_refl H23 H14); dest.
+          derive_child_st rcidx.
+          disc_MsgConflictsInv rcidx.
+          rewrite H49 in H44; simpl in H44; dest.
+          solve_ObjsInvalid_trivial.
+
+          eapply ObjsInvalid_in_composed; eauto.
+          { left; repeat split; [simpl; solve_mesi|simpl; rewrite H58; discriminate|].
+            apply NoCohMsgs_rsUps_deq; eauto.
+            { eapply Forall_impl; [|apply Hrss].
+              simpl; intros; dest; eauto.
+            }
+            { apply in_map with (f:= idOf) in H40; assumption. }
+            { rewrite Forall_forall in H17; specialize (H17 _ H40).
+              eapply NoCohMsgs_rsUp_deq; eauto.
+            }
+          }
+          { eapply ObjsInvalid_this_rsUps_deqMsgs_silent; eauto.
+            intro Hx; destruct Hx as [ccidx [? ?]].
+            eapply subtreeIndsOf_child_SubList in H60; eauto.
+            apply parent_not_in_subtree in H37; auto.
+          }
+        }
+        { disc_InvExcl oidx.
+          specialize (H40 (tl_In _ _ H8)).
+          move H40 at bottom.
+          specialize (H40 _ H37); destruct H40 as [? _].
+          specialize (H40 Hcs).
+          solve_ObjsInvalid_trivial.
+          eapply ObjsInvalid_this_rsUps_deqMsgs_silent with (pidx:= oidx); eauto.
+          intro; solve_by_topo_false.
+        }
+      }
+
+      assert (NoRsI oidx msgs) as Hrsi.
+      { move Hidir at bottom.
+        specialize (Hidir oidx); simpl in Hidir.
+        rewrite H15 in Hidir; simpl in Hidir.
+        eapply not_MsgExistsSig_MsgsNotExist; intros;
+          inv H37; [|dest_in].
+        specialize (Hidir (or_intror (or_intror H38))).
+        simpl in *; solve_mesi.
+      }
+
+      (** 2-2) ObjsInvalid, outside [oidx] *)
+      assert (forall nost rsTo,
+                 ObjsInvalid
+                   (fun idx => ~ In idx (subtreeIndsOf (fst (tree2Topo tr 0)) oidx))
+                   (oss +[oidx <- nost])
+                   (enqMP (downTo x) rsTo (deqMsgs (idsOf rins) msgs))) as Hoo.
+      { intros.
+        solve_ObjsInvalid_trivial.
+        eapply ObjsInvalid_this_rsUps_deqMsgs_silent with (pidx:= oidx); eauto;
+          [|intro; solve_by_topo_false].
+        disc_InvExcl oidx.
+        destruct H28; simpl in *; dest.
+        { specialize (H37 (conj H28 Hrsi)); dest; assumption. }
+        { specialize (H38 (tl_In _ _ H8)).
+          apply subtreeChildrenIndsOf_parentIdxOf in H39; auto.
+          specialize (H38 _ H39); destruct H38 as [_ ?].
+          rewrite getDir_excl_eq in H38; [|reflexivity|intuition solve_mesi].
+          specialize (H38 H28).
+          eapply ObjsInvalid_impl; [eassumption|].
+          simpl; intros.
+          intro Hx; elim H42.
+          eapply subtreeIndsOf_child_SubList with (cidx:= dir_excl _); eauto.
+        }
+      }
+
+      (** 2-3) The target object itself gets invalid *)
+      assert (forall rsTo,
+                 ObjInvalid0
+                   oidx (fst os,
+                         (false,
+                          (mesiI, (setDirM x, snd (snd (snd (snd os)))))))
+                   (enqMP (downTo x) rsTo (deqMsgs (idsOf rins) msgs))) as Hoi.
+      { intros; repeat split; [simpl; reflexivity|discriminate|].
+        disc_InvExcl oidx.
+        destruct H28; simpl in *; dest.
+        { specialize (H37 (conj H28 Hrsi)); dest; solve_MsgsP. }
+        { specialize (H38 (tl_In _ _ H8)).
+          apply subtreeChildrenIndsOf_parentIdxOf in H39; auto.
+          specialize (H38 _ H39); destruct H38 as [_ ?].
+          rewrite getDir_excl_eq in H38; [|reflexivity|intuition solve_mesi].
+          specialize (H38 H28).
+          apply parent_not_in_subtree in H39; auto.
+          specialize (H38 _ H39).
+          rewrite H15 in H38; simpl in H38.
+          solve_MsgsP.
+          disc_MsgConflictsInv oidx.
+          eapply ObjInvalid_NoCohMsgs; eauto.
+        }
+      }
+
+      (** 3) Predicate for [mesiRsM] *)
+      assert (ObjsInvalid
+                (fun idx => ~ In idx (subtreeIndsOf (fst (tree2Topo tr 0)) x))
+                (oss +[oidx <- (fst os,
+                                (false,
+                                 (mesiI, (setDirM x, snd (snd (snd (snd os)))))))])
+                (enqMP (downTo x)
+                       {| msg_id := mesiRsM;
+                          msg_type := MRs;
+                          msg_value := 0 |} (deqMsgs (idsOf rins) msgs))) as Hrc.
+      { intros.
+        eapply ObjsInvalid_out_composed with (oidx:= oidx); eauto.
+        { mred. }
+        { left; apply Hoi. }
+      }
+
+      split.
+      { solve_AtomicInv_rsUps_rsDown Hrsd.
+        red; simpl; intros; inv H37.
+        rewrite <-H13; eapply Hrc.
+      }
+
+      { case_InvExcl_me_others.
+        { disc_InvExcl_this.
+          { solve_InvObjExcl0_by_ObjExcl0_false. }
+          { solve_InvObjOwned_by_false. }
+          { split_InvDirInv.
+            { case_idx_eq x cidx;
+                [rewrite getDir_setDirM_eq in H41; discriminate|clear H41].
+              rewrite <-H13; eapply Hcsi; eauto.
+            }
+            { case_idx_eq x cidx;
+                [clear H41
+                |simpl in H41; rewrite getDir_setDirM_neq in H41 by assumption;
+                 solve_mesi].
+              rewrite <-H13; eapply Hrc.
+            }
+          }
+        }
+
+        { destruct H28; dest; [solve_mesi|].
+          pose proof Hpmcf as Hpmcf'; phide Hpmcf'; rename H40 into Hpmcf'.
           disc_MsgConflictsInv oidx.
 
-          pick_rsUps_one.
+          remember (dir_excl _) as cidx; clear Heqcidx.
+          rewrite H38 in H13.
+          destruct rins as [|[midx rmsg] rins]; [discriminate|].
+          destruct rins; [|discriminate].
+          simpl in H13; inv H13.
+
           (* discharge all predicates in [Forall] *)
-          inv H14; inv H17; inv H23; dest; simpl in *.
+          inv H14; inv H17; inv H23; inv Hrss; dest; simpl in *.
+          clear H47 H48 H49 H50. (* [Forall _ nil] *)
+          inv H14; rename x0 into cidx.
           derive_child_chns cidx; repeat disc_rule_minds.
           (* derive the predicate message for it *)
           apply SubList_cons_inv in H3; dest.
@@ -5895,51 +6624,38 @@ Section InvExcl.
 
           disc_InvExcl_others.
           { disc_InvObjExcl0.
-            rewrite <-H13 in H73; simpl in H73.
-            change (deqMsgs (idsOf rins) (deqMP (rsUpFrom cidx) msgs))
-              with (deqMsgs (idsOf ((rsUpFrom cidx, msg0) :: rins)) msgs) in H73.
-            apply ObjExcl0_other_msg_id_deqMsgs_inv in H73; auto.
-            2: { constructor; simpl; [rewrite H50; discriminate|].
-                 eapply Forall_impl; [|apply H51]; simpl; intros.
-                 rewrite H74; discriminate.
-            }
-            specialize (H4 H73); dest.
-
-            clear H67.
+            rewrite H38 in H71; simpl in H71.
+            eapply ObjExcl0_other_msg_id_deqMP_inv in H71; eauto;
+              [|simpl; rewrite H46; discriminate].
+            specialize (H4 H71); dest.
             exfalso.
             case_idx_eq eidx cidx.
             { disc_rule_conds_ex; disc_ObjExcl0; solve_mesi. }
-            { solve_by_ObjsInvalid_downRsI_false cidx. }
+            { solve_by_ObjsInvalid_downRsIM_false cidx. }
           }
 
           { red; intros [? ?].
             assert (NoRsI eidx msgs).
-            { disc_MsgsP H74.
-              rewrite <-H13 in H74; simpl in H74.
-              change (deqMsgs (idsOf rins) (deqMP (rsUpFrom cidx) msgs))
-                with (deqMsgs (idsOf ((rsUpFrom cidx, msg0) :: rins)) msgs) in H74.
-              apply MsgsP_other_msg_id_deqMsgs_inv in H74; auto.
-              simpl; apply (DisjList_spec_2 idx_dec); intros; dest_in.
-              intro; dest_in; [rewrite H50 in H76; discriminate|].
-              apply in_map_iff in H76; destruct H76 as [[rmidx rmsg] [? ?]]; simpl in *.
-              rewrite Forall_forall in H51; specialize (H51 _ H76); simpl in *.
-              rewrite H51 in H75; discriminate.
+            { disc_MsgsP H72.
+              rewrite H38 in H72; simpl in H72.
+              eapply MsgsP_other_msg_id_deqMP_inv in H72; eauto.
+              simpl; rewrite H46; intuition discriminate.
             }
-            specialize (H71 (conj H73 H75)); dest.
+            specialize (H69 (conj H71 H73)); dest.
 
-            case_in_subtree cidx eidx; [|solve_by_ObjsInvalid_downRsI_false cidx].
-            case_idx_eq eidx cidx; [disc_rule_conds_ex; congruence|].
+            case_in_subtree cidx eidx; [|solve_by_ObjsInvalid_downRsIM_false cidx].
+            case_idx_eq eidx cidx; [disc_rule_conds_ex; congruence (* owner true/false *) |].
             split.
             { assert (In oidx (subtreeIndsOf (fst (tree2Topo tr 0)) eidx)).
               { eapply inside_parent_in with (cidx:= cidx); eauto. }
               solve_ObjsInvalid_trivial.
-              rewrite <-H13.
+              rewrite H38.
               eapply ObjsInvalid_this_rsUps_deqMsgs_silent with (pidx:= oidx); eauto.
             }
             { case_idx_eq x eidx; [|solve_MsgsP].
               assert (~ In cidx (subtreeIndsOf (fst (tree2Topo tr 0)) eidx)).
               { intro; solve_by_topo_false. }
-              solve_by_ObjsInvalid_downRsI_false cidx.
+              solve_by_ObjsInvalid_downRsIM_false cidx.
             }
           }
 
@@ -5950,22 +6666,22 @@ Section InvExcl.
                 { eapply inside_parent_in with (cidx:= x); eauto. }
                 assert (In cidx (subtreeIndsOf (fst (tree2Topo tr 0)) cidx0)).
                 { eapply inside_child_in; eauto. }
-                solve_by_ObjsInvalid_downRsI_false cidx.
+                solve_by_ObjsInvalid_downRsIM_false cidx.
               }
-              { case_in_subtree cidx cidx0; [solve_by_ObjsInvalid_downRsI_false cidx|].
+              { case_in_subtree cidx cidx0; [solve_by_ObjsInvalid_downRsIM_false cidx|].
                 solve_ObjsInvalid_trivial.
-                rewrite <-H13.
+                rewrite H38.
                 eapply ObjsInvalid_this_rsUps_deqMsgs_silent with (pidx:= oidx); eauto.
                 intro; solve_by_topo_false.
               }
             }
             { case_in_subtree cidx cidx0;
-                [|solve_by_ObjsInvalid_downRsI_false cidx].
+                [|solve_by_ObjsInvalid_downRsIM_false cidx].
               case_idx_eq cidx cidx0; [disc_rule_conds|].
               assert (In oidx (subtreeIndsOf (fst (tree2Topo tr 0)) cidx0)).
               { eapply inside_parent_in with (cidx:= cidx); eauto. }
               solve_ObjsInvalid_trivial.
-              rewrite <-H13.
+              rewrite H38.
               eapply ObjsInvalid_this_rsUps_deqMsgs_silent with (pidx:= oidx); eauto.
             }
           }
@@ -5973,7 +6689,7 @@ Section InvExcl.
       }
     }
 
-    { (* [liDownIImm] *)
+    { (* [liDownIImmS] *)
       disc_rule_conds_ex.
       derive_NoRsI_by_rqDown oidx msgs.
 
@@ -5985,7 +6701,7 @@ Section InvExcl.
         { simpl in *; inv H17; mred.
           disc_MsgConflictsInv oidx0.
           disc_InvExcl oidx0.
-          eapply ObjsInvalid_downRsI; eauto.
+          eapply ObjsInvalid_downRsIS; eauto.
           { apply tl_In; assumption. }
           { assumption. }
         }
@@ -6002,6 +6718,63 @@ Section InvExcl.
         }
         { disc_InvExcl_others.
           { disc_InvObjExcl0_apply.
+            split; [|solve_MsgsP].
+            solve_ObjsInvalid_trivial.
+            eapply ObjsInvalid_state_transition_sound; eauto.
+          }
+          { disc_InvObjOwned.
+            split; [|solve_MsgsP].
+            solve_ObjsInvalid_trivial.
+            eapply ObjsInvalid_state_transition_sound; eauto.
+          }
+          { split_InvDirInv_apply.
+            { case_in_subtree oidx cidx.
+              { solve_ObjsInvalid_trivial.
+                eapply ObjsInvalid_state_transition_sound; eauto.
+              }
+              { solve_ObjsInvalid_trivial. }
+            }
+            { case_in_subtree oidx cidx.
+              { solve_ObjsInvalid_trivial. }
+              { solve_ObjsInvalid_trivial.
+                eapply ObjsInvalid_state_transition_sound; eauto.
+              }
+            }
+          }
+        }
+      }
+    }
+
+    { (* [liDownIImmME] *)
+      disc_rule_conds_ex.
+      derive_NoRsI_by_rqDown oidx msgs.
+
+      split.
+      { solve_AtomicInv_rqDown_rsUp.
+        { simpl in *; inv H17; mred.
+          simpl; intuition solve_mesi.
+        }
+        { simpl in *; inv H17; mred.
+          disc_MsgConflictsInv oidx0.
+          disc_InvExcl oidx0.
+          eapply ObjsInvalid_downRsIM; eauto.
+          { apply tl_In; assumption. }
+          { assumption. }
+        }
+      }
+
+      { case_InvExcl_me_others.
+        { disc_InvExcl_this.
+          { solve_InvObjExcl0_by_ObjExcl0_false. }
+          { solve_InvObjOwned_by_false. }
+          { split_InvDirInv_apply.
+            { solve_ObjsInvalid_trivial. }
+            { exfalso; disc_dir; solve_mesi. }
+          }
+        }
+        { disc_InvExcl_others.
+          { disc_InvObjExcl0_apply.
+            disc_MsgConflictsInv oidx.
             solve_by_ObjsInvalid_status_false oidx.
           }
           { case_InvObjOwned.
@@ -6055,7 +6828,7 @@ Section InvExcl.
       { solve_InvExcl_trivial. }
     }
 
-    { (* [liDownIRsUpUp] *)
+    { (* [liDownIRsUpUpS] *)
       disc_rule_conds_ex.
       disc_MesiDownLockInv oidx Hdlinv.
       derive_footprint_info_basis oidx; [solve_midx_false|].
@@ -6068,8 +6841,8 @@ Section InvExcl.
                      midx = rsUpFrom rcidx)
                 (idsOf rins)) as Hrss.
       { apply Forall_forall; intros rsUp ?.
-        eapply RqRsDownMatch_rs_rq in H31; [|rewrite <-H13; eassumption].
-        destruct H31 as [cidx [down ?]]; dest.
+        eapply RqRsDownMatch_rs_rq in H33; [|rewrite <-H13; eassumption].
+        destruct H33 as [cidx [down ?]]; dest.
         derive_child_chns cidx; repeat disc_rule_minds.
         eauto.
       }
@@ -6081,19 +6854,11 @@ Section InvExcl.
                  then True
                  else getDir rcidx os#[dir] = mesiI) as Hcs.
       { intros.
-        destruct H27; simpl in *; dest.
-        { destruct (in_dec idx_dec rcidx (dir_sharers (fst (snd (snd (snd os)))))).
-          { find_if_inside; [auto|].
-            elim n; rewrite H13, H32; apply in_map; assumption.
-          }
-          { find_if_inside; [auto|apply getDir_S_non_sharer; assumption]. }
+        destruct (in_dec idx_dec rcidx (dir_sharers (fst (snd (snd (snd os)))))).
+        { find_if_inside; [auto|].
+          elim n; rewrite H13, H29; apply in_map; assumption.
         }
-        { case_idx_eq rcidx (dir_excl (fst (snd (snd (snd os))))).
-          { find_if_inside; [auto|].
-            elim n; rewrite H13, H32; left; reflexivity.
-          }
-          { find_if_inside; [auto|erewrite getDir_excl_neq; eauto]. }
-        }
+        { find_if_inside; [auto|apply getDir_S_non_sharer; assumption]. }
       }
 
       (** 2-2) Each child subtree satisfies [ObjsInvalid] *)
@@ -6106,62 +6871,76 @@ Section InvExcl.
                      (oss +[oidx <- nost])
                      (enqMP (rsUpFrom oidx) rsTo (deqMsgs (idsOf rins) msgs))) as Hcsi.
       { intros.
-        specialize (Hcs _ H29); find_if_inside.
+        specialize (Hcs _ H31); find_if_inside.
         { apply in_map_iff in i; destruct i as [[midx rs] ?]; simpl in *; dest; subst.
-          rewrite Forall_forall in H14; specialize (H14 _ H32).
-          rewrite Forall_forall in H23; specialize (H23 _ H32); simpl in *.
-          pose proof (H3 _ H32) as Hrein.
+          rewrite Forall_forall in H14; specialize (H14 _ H34).
+          rewrite Forall_forall in H23; specialize (H23 _ H34); simpl in *.
+          pose proof (H3 _ H34) as Hrein.
           disc_AtomicMsgOutsInv rcidx.
-          specialize (H36 eq_refl H23 H14); dest.
+          specialize (H38 eq_refl H23 H14); dest.
           derive_child_st rcidx.
           disc_MsgConflictsInv rcidx.
-          rewrite H41 in H36; simpl in H36; dest.
+          rewrite H44 in H38; simpl in H38; dest.
           solve_ObjsInvalid_trivial.
-
-          eapply ObjsInvalid_in_composed; eauto.
-          { left; split; [simpl; solve_mesi|].
-            apply NoCohMsgs_rsUps_deq; eauto.
-            { eapply Forall_impl; [|apply Hrss].
-              simpl; intros; dest; eauto.
-            }
-            { apply in_map with (f:= idOf) in H32; assumption. }
-            { rewrite Forall_forall in H17; specialize (H17 _ H32).
-              eapply NoCohMsgs_rsUp_deq; eauto.
-            }
-          }
-          { eapply ObjsInvalid_this_rsUps_deqMsgs_silent; eauto.
-            intro Hx; destruct Hx as [ccidx [? ?]].
-            eapply subtreeIndsOf_child_SubList in H52; eauto.
-            apply parent_not_in_subtree in H52; auto.
-          }
+          eapply ObjsInvalid_this_rsUps_deqMsgs_silent; eauto.
+          apply parent_not_in_subtree; auto.
         }
         { disc_InvExcl oidx.
-          specialize (H32 (tl_In _ _ H8)).
-          move H32 at bottom.
-          specialize (H32 _ H29); destruct H32 as [? _].
-          specialize (H32 Hcs).
+          specialize (H34 (tl_In _ _ H8)).
+          move H34 at bottom.
+          specialize (H34 _ H31); destruct H34 as [? _].
+          specialize (H34 Hcs).
           solve_ObjsInvalid_trivial.
           eapply ObjsInvalid_this_rsUps_deqMsgs_silent with (pidx:= oidx); eauto.
           intro; solve_by_topo_false.
         }
       }
 
-      (** 3) Predicate for [mesiDownRsI] *)
-      assert (forall nost rsTo,
-                 ObjsInvalid
-                   (fun idx =>
-                      exists cidx,
-                        parentIdxOf (fst (tree2Topo tr 0)) cidx = Some oidx /\
-                        In idx (subtreeIndsOf (fst (tree2Topo tr 0)) cidx))
-                   (oss +[oidx <- nost])
-                   (enqMP (rsUpFrom oidx) rsTo (deqMsgs (idsOf rins) msgs))) as Hrc.
-      { intros; eapply ObjsInvalid_downRsI_composed; [mred|eauto]. }
+      (** 2-3) The target object itself gets invalid *)
+      assert (ObjInvalid0
+                oidx (fst os, (false, (mesiI, (setDirI, snd (snd (snd (snd os)))))))
+                (enqMP (rsUpFrom oidx)
+                       {| msg_id := mesiDownRsIS; msg_type := MRs; msg_value := 0 |}
+                       (deqMsgs (idsOf rins) msgs))) as Hoi.
+      { intros; repeat split; [simpl; reflexivity|discriminate|].
+        clear Hpmcf; preveal Hnmcf.
+        assert ((orqs +[oidx <- porq -[downRq]])@[oidx] = Some (porq -[downRq]))
+          by mred.
+        disc_MsgConflictsInv oidx.
+        rewrite H13.
+        eapply NoCohMsgs_rsUp_in; eauto.
+        { apply InMP_or_enqMP; left; auto. }
+        { discriminate. }
+        { discriminate. }
+      }
+
+      (** 3) Predicate for [mesiDownRsIS] *)
+      assert (ObjsInvalid
+                (fun idx => In idx (subtreeIndsOf (fst (tree2Topo tr 0)) oidx))
+                (oss +[oidx <- (fst os, (false, (mesiI, (setDirI, snd (snd (snd (snd os)))))))])
+                (enqMP (rsUpFrom oidx)
+                       {| msg_id := mesiDownRsIS; msg_type := MRs; msg_value := 0 |}
+                       (deqMsgs (idsOf rins) msgs))) as Hrc.
+      { eapply ObjsInvalid_in_composed; [mred|..].
+        { left; apply Hoi. }
+        { intros; eapply ObjsInvalid_downRsIM_composed; [mred|eauto]. }
+      }
+
+      assert (NoRsI oidx msgs) as Hrsi.
+      { move Hidir at bottom.
+        specialize (Hidir oidx); simpl in Hidir.
+        rewrite H15 in Hidir; simpl in Hidir.
+        eapply not_MsgExistsSig_MsgsNotExist; intros;
+          inv H31; [|dest_in].
+        specialize (Hidir (or_intror (or_intror H32))).
+        simpl in *; solve_mesi.
+      }
 
       split.
       { rewrite <-H13.
         solve_AtomicInv_rsUps_rsUp.
-        { simpl in *; inv H29; mred; simpl; intuition solve_mesi. }
-        { simpl in *; inv H29; apply Hrc. }
+        { simpl in *; inv H31; mred; simpl; intuition solve_mesi. }
+        { simpl in *; inv H31; apply Hrc. }
       }
 
       { case_InvExcl_me_others.
@@ -6171,91 +6950,223 @@ Section InvExcl.
           { split_InvDirInv.
             { rewrite <-H13; eapply Hcsi; eauto. }
             { exfalso.
-              simpl in H35; rewrite getDir_setDirI in H35.
+              simpl in H37; rewrite getDir_setDirI in H37.
               solve_mesi.
             }
           }
         }
 
-        { pose proof Hpmcf as Hpmcf'; phide Hpmcf'; rename H29 into Hpmcf'.
-          disc_MsgConflictsInv oidx.
-
-          pick_rsUps_one.
-          (* discharge all predicates in [Forall] *)
-          inv H14; inv H17; inv H23; dest; simpl in *.
-          derive_child_chns cidx; repeat disc_rule_minds.
-          (* derive the predicate message for it *)
-          apply SubList_cons_inv in H3; dest.
-          disc_AtomicMsgOutsInv cidx.
-
-          derive_child_st cidx.
-          disc_MsgPred.
-          preveal Hpmcf'; disc_MsgConflictsInv cidx.
-
-          disc_InvExcl_others.
+        { disc_InvExcl_others.
           { disc_InvObjExcl0.
-            rewrite <-H13 in H67; simpl in H67.
-            change (deqMsgs (idsOf rins) (deqMP (rsUpFrom cidx) msgs))
-              with (deqMsgs (idsOf ((rsUpFrom cidx, msg0) :: rins)) msgs) in H67.
-            apply ObjExcl0_other_msg_id_deqMsgs_inv in H67; auto.
-            2: { constructor; simpl; [rewrite H43; discriminate|].
-                 eapply Forall_impl; [|apply H44]; simpl; intros.
-                 rewrite H68; discriminate.
+            rewrite <-H13 in H35.
+            apply ObjExcl0_other_msg_id_deqMsgs_inv in H35; auto.
+            2: { eapply Forall_impl; [|apply H14]; simpl; intros.
+                 rewrite H36; discriminate.
             }
-            specialize (H4 H67); dest.
-
-            clear H61.
+            specialize (H4 H35); dest.
             exfalso.
-            case_idx_eq eidx cidx.
-            { disc_rule_conds; disc_ObjExcl0; solve_mesi. }
-            { solve_by_ObjsInvalid_downRsI_false cidx. }
+            disc_ObjsInvalid_by oidx.
+            rewrite H15 in H37; simpl in H37.
+            destruct H37.
+            { destruct H37 as [? [? ?]]; auto. }
+            { eapply NoRsI_MsgExistsSig_InvRs_false; eauto. }
           }
+
           { red; intros [? ?].
             assert (NoRsI eidx msgs).
-            { disc_MsgsP H68.
-              rewrite <-H13 in H68; simpl in H68.
-              change (deqMsgs (idsOf rins) (deqMP (rsUpFrom cidx) msgs))
-                with (deqMsgs (idsOf ((rsUpFrom cidx, msg0) :: rins)) msgs) in H68.
-              apply MsgsP_other_msg_id_deqMsgs_inv in H68; auto.
+            { disc_MsgsP H36.
+              rewrite <-H13 in H36; simpl in H36.
+              apply MsgsP_other_msg_id_deqMsgs_inv in H36; auto.
               simpl; apply (DisjList_spec_2 idx_dec); intros; dest_in.
-              intro; dest_in; [rewrite H43 in H70; discriminate|].
-              apply in_map_iff in H70; destruct H70 as [[rmidx rmsg] [? ?]]; simpl in *.
-              rewrite Forall_forall in H44; specialize (H44 _ H70); simpl in *.
-              rewrite H44 in H69; discriminate.
+              intro; dest_in.
+              apply in_map_iff in H37; destruct H37 as [[rmidx rmsg] [? ?]]; simpl in *.
+              rewrite Forall_forall in H14; specialize (H14 _ H38); simpl in *.
+              rewrite H14 in H37; discriminate.
             }
-            specialize (H65 (conj H67 H69)); dest.
+            specialize (H32 (conj H35 H37)); dest.
 
-            case_in_subtree cidx eidx; [|solve_by_ObjsInvalid_downRsI_false cidx].
-            case_idx_eq eidx cidx; [disc_rule_conds_ex; congruence|].
+            case_in_subtree oidx eidx;
+              [|clear Hrc; solve_by_ObjsInvalid_dir_false oidx].
             split.
-            { assert (In oidx (subtreeIndsOf (fst (tree2Topo tr 0)) eidx)).
-              { eapply inside_parent_in with (cidx:= cidx); eauto. }
-              solve_ObjsInvalid_trivial.
+            { solve_ObjsInvalid_trivial.
               rewrite <-H13.
               eapply ObjsInvalid_this_rsUps_deqMsgs_silent with (pidx:= oidx); eauto.
             }
             { solve_MsgsP. }
           }
+
           { split_InvDirInv_apply.
-            { case_in_subtree oidx cidx0.
-              { assert (In cidx (subtreeIndsOf (fst (tree2Topo tr 0)) cidx0)).
-                { eapply inside_child_in; eauto. }
-                solve_by_ObjsInvalid_downRsI_false cidx.
-              }
-              { case_in_subtree cidx cidx0; [solve_by_ObjsInvalid_downRsI_false cidx|].
-                solve_ObjsInvalid_trivial.
+            { case_in_subtree oidx cidx.
+              { clear Hrc; solve_by_ObjsInvalid_dir_false oidx. }
+              { solve_ObjsInvalid_trivial.
                 rewrite <-H13.
                 eapply ObjsInvalid_this_rsUps_deqMsgs_silent with (pidx:= oidx); eauto.
               }
             }
-            { case_in_subtree cidx cidx0;
-                [|solve_by_ObjsInvalid_downRsI_false cidx].
-              case_idx_eq cidx cidx0; [disc_rule_conds|].
-              assert (In oidx (subtreeIndsOf (fst (tree2Topo tr 0)) cidx0)).
-              { eapply inside_parent_in with (cidx:= cidx); eauto. }
+            { case_in_subtree oidx cidx.
+              { solve_ObjsInvalid_trivial.
+                rewrite <-H13.
+                eapply ObjsInvalid_this_rsUps_deqMsgs_silent with (pidx:= oidx); eauto.
+              }
+              { clear Hrc; solve_by_ObjsInvalid_dir_false oidx. }
+            }
+          }
+        }
+      }
+    }
+
+    { (* [liDownIRsUpUpME] *)
+      disc_rule_conds_ex.
+      disc_MesiDownLockInv oidx Hdlinv.
+      derive_footprint_info_basis oidx; [solve_midx_false|].
+
+      (** 1) Each RsUp message is from a child *)
+      assert (Forall
+                (fun midx =>
+                   exists rcidx,
+                     parentIdxOf (fst (tree2Topo tr 0)) rcidx = Some oidx /\
+                     midx = rsUpFrom rcidx)
+                (map fst (rqi_rss rqi))) as Hrss.
+      { apply Forall_forall; intros rsUp ?.
+        eapply RqRsDownMatch_rs_rq in H34; [|eassumption].
+        destruct H34 as [cidx [down ?]]; dest.
+        derive_child_chns cidx; repeat disc_rule_minds.
+        eauto.
+      }
+
+      (** 2-1) Each child either sent RsUp or is in DirI *)
+      assert (forall rcidx,
+                 parentIdxOf (fst (tree2Topo tr 0)) rcidx = Some oidx ->
+                 if in_dec idx_dec (rsUpFrom rcidx) (map fst (rqi_rss rqi))
+                 then True
+                 else getDir rcidx os#[dir] = mesiI) as Hcs.
+      { intros.
+        find_if_inside; [auto|].
+        rewrite <-H13 in n.
+        eapply getDir_excl_neq; eauto.
+        intro Hx; subst.
+        elim n; left; reflexivity.
+      }
+
+      remember (dir_excl _) as ecidx; clear Heqecidx.
+      apply subtreeChildrenIndsOf_parentIdxOf in H28; auto.
+
+      (** 2-2) Each child subtree satisfies [ObjsInvalid] *)
+      assert (forall rcidx,
+                 parentIdxOf (fst (tree2Topo tr 0)) rcidx = Some oidx ->
+                 forall nost rsTo,
+                   ObjsInvalid
+                     (fun idx =>
+                        In idx (subtreeIndsOf (fst (tree2Topo tr 0)) rcidx))
+                     (oss +[oidx <- nost])
+                     (enqMP (rsUpFrom oidx) rsTo (deqMP (rsUpFrom ecidx) msgs)))
+        as Hcsi.
+      { intros.
+        specialize (Hcs _ H23); find_if_inside.
+        { rewrite <-H13 in i; dest_in; inv H33.
+          disc_AtomicMsgOutsInv rcidx.
+          specialize (H39 eq_refl H32 H31); dest.
+          derive_child_st rcidx.
+          disc_MsgConflictsInv rcidx.
+          rewrite H44 in H39; simpl in H39; dest.
+          solve_ObjsInvalid_trivial.
+
+          eapply ObjsInvalid_in_composed; eauto.
+          { left; repeat split; [simpl; solve_mesi|intro Hx; simpl in Hx; solve_mesi|].
+            eapply NoCohMsgs_rsUp_deq; eauto.
+          }
+          { eapply ObjsInvalid_this_rsUps_deqMsgs_silent with (rminds := [_]); eauto.
+            intro Hx; destruct Hx as [ccidx [? ?]].
+            eapply subtreeIndsOf_child_SubList in H55; eauto.
+            eapply parent_not_in_subtree in H55; eauto.
+          }
+        }
+        { disc_InvExcl oidx.
+          specialize (H35 (tl_In _ _ H8)).
+          move H35 at bottom.
+          specialize (H35 _ H23); destruct H35 as [? _].
+          specialize (H35 Hcs).
+          solve_ObjsInvalid_trivial.
+          eapply ObjsInvalid_this_rsUps_deqMsgs_silent with (pidx:= oidx) (rminds:= [_]); eauto.
+          intro; solve_by_topo_false.
+        }
+      }
+
+      (** 3) Predicate for [mesiDownRsIM] *)
+      assert (forall nost rsTo,
+                 ObjsInvalid
+                   (fun idx =>
+                      exists cidx,
+                        parentIdxOf (fst (tree2Topo tr 0)) cidx = Some oidx /\
+                        In idx (subtreeIndsOf (fst (tree2Topo tr 0)) cidx))
+                   (oss +[oidx <- nost])
+                   (enqMP (rsUpFrom oidx) rsTo (deqMP (rsUpFrom ecidx) msgs))) as Hrc.
+      { intros; eapply ObjsInvalid_downRsIM_composed; [mred|eauto]. }
+
+      split.
+      { solve_AtomicInv_rsUps_rsUp.
+        { simpl in *; inv H23; mred; simpl; intuition solve_mesi. }
+        { simpl in *; inv H23; apply Hrc. }
+      }
+
+      { case_InvExcl_me_others.
+        { disc_InvExcl_this.
+          { solve_InvObjExcl0_by_ObjExcl0_false. }
+          { solve_InvObjOwned_by_false. }
+          { split_InvDirInv.
+            { eapply Hcsi; eauto. }
+            { exfalso.
+              simpl in H38; rewrite getDir_setDirI in H38.
+              solve_mesi.
+            }
+          }
+        }
+
+        { pose proof Hpmcf as Hpmcf'; phide Hpmcf'; rename H23 into Hpmcf'.
+          disc_MsgConflictsInv oidx.
+
+          (* discharge all predicates in [Forall] *)
+          derive_child_chns ecidx; repeat disc_rule_minds.
+          (* derive the predicate message for it *)
+          disc_AtomicMsgOutsInv ecidx.
+
+          derive_child_st ecidx.
+          disc_MsgPred.
+          preveal Hpmcf'; disc_MsgConflictsInv ecidx.
+
+          disc_InvExcl_others.
+          { disc_InvObjExcl0_apply.
+            exfalso.
+            case_idx_eq eidx ecidx.
+            { disc_rule_conds; disc_ObjExcl0; solve_mesi. }
+            { solve_by_ObjsInvalid_downRsIM_false ecidx. }
+          }
+          { disc_InvObjOwned.
+            case_in_subtree ecidx eidx; [|solve_by_ObjsInvalid_downRsIM_false ecidx].
+            case_idx_eq eidx ecidx; [disc_rule_conds_ex; congruence|].
+            split.
+            { assert (In oidx (subtreeIndsOf (fst (tree2Topo tr 0)) eidx)).
+              { eapply inside_parent_in with (cidx:= ecidx); eauto. }
               solve_ObjsInvalid_trivial.
-              rewrite <-H13.
-              eapply ObjsInvalid_this_rsUps_deqMsgs_silent with (pidx:= oidx); eauto.
+            }
+            { solve_MsgsP. }
+          }
+          { split_InvDirInv_apply.
+            { case_in_subtree oidx cidx.
+              { assert (In ecidx (subtreeIndsOf (fst (tree2Topo tr 0)) cidx)).
+                { eapply inside_child_in; eauto. }
+                solve_by_ObjsInvalid_downRsIM_false ecidx.
+              }
+              { case_in_subtree ecidx cidx; [solve_by_ObjsInvalid_downRsIM_false ecidx|].
+                solve_ObjsInvalid_trivial.
+              }
+            }
+            { case_in_subtree ecidx cidx;
+                [|solve_by_ObjsInvalid_downRsIM_false ecidx].
+              case_idx_eq ecidx cidx; [disc_rule_conds|].
+              assert (In oidx (subtreeIndsOf (fst (tree2Topo tr 0)) cidx)).
+              { eapply inside_parent_in with (cidx:= ecidx); eauto. }
+              solve_ObjsInvalid_trivial.
             }
           }
         }
@@ -6279,6 +7190,17 @@ Section InvExcl.
       derive_footprint_info_basis oidx.
       disc_MsgConflictsInv oidx.
 
+      assert (os#[dir].(dir_st) = mesiI) as Hdir.
+      { move Hidir at bottom.
+        specialize (Hidir oidx); simpl in Hidir.
+        rewrite H15 in Hidir; simpl in Hidir.
+        apply Hidir.
+        do 2 right.
+        exists (downTo oidx, rmsg); split.
+        { apply FirstMP_InMP; assumption. }
+        { unfold sigOf; simpl; congruence. }
+      }
+
       split.
       { solve_AtomicInv_rsDown. }
       { case_InvExcl_me_others.
@@ -6300,7 +7222,7 @@ Section InvExcl.
           }
           { case_InvObjOwned.
             { left.
-              red; simpl; split; [solve_mesi|].
+              red; simpl; repeat split; [solve_mesi|rewrite Hdir; discriminate|].
               eapply NoCohMsgs_rsDown_deq; eauto.
             }
             { disc_ObjsInvalid_by oidx0.
@@ -6336,7 +7258,7 @@ Section InvExcl.
     Unshelve.
     all: assumption.
 
-    (* END_SKIP_PROOF_OFF *)
+    END_SKIP_PROOF_ON *) admit.
   Qed.
 
   Lemma mesi_InvExcl_InvTrs_l1:
@@ -6363,12 +7285,13 @@ Section InvExcl.
               AtomicInv InvExclMsgOutPred inits ist1 (RlblInt oidx ridx rins routs :: hst)
                         (removeL (id_dec msg_dec) eouts rins ++ routs) ist2 /\
               InvExcl topo cifc ist2.
-  Proof. (* SKIP_PROOF_OFF *)
+  Proof. (* SKIP_PROOF_ON
     intros.
     pose proof (tree2Topo_TreeTopoNode tr 0) as Htn.
     pose proof (footprints_ok
                   (mesi_GoodORqsInit Htr)
                   (mesi_GoodRqRsSys Htr) Hr1) as Hftinv.
+    pose proof (mesi_InvL1DirI_ok Hr1) as Hdiri.
     pose proof (mesi_InObjInds Hr1) as Hioi1.
     pose proof (mesi_InObjInds Hr2) as Hioi2.
     pose proof (mesi_OstInds Hr1) as Hosi.
@@ -6645,7 +7568,7 @@ Section InvExcl.
       }
     }
 
-    { (* [l1DownIImm] *)
+    { (* [l1DownIImmS] *)
       disc_rule_conds_ex.
       derive_NoRsI_by_rqDown oidx msgs.
 
@@ -6654,6 +7577,74 @@ Section InvExcl.
         solve_AtomicInv_rqDown_rsUp.
         { simpl in *; inv H31; mred.
           simpl; intuition solve_mesi.
+        }
+        { simpl in *; inv H31; mred.
+          eapply ObjsInvalid_in_composed; [mred|..].
+          { left; repeat split; [simpl; solve_mesi|..].
+            { Ltac disc_InvL1DirI oidx :=
+                match goal with
+                | [Hdiri: InvL1DirI _ _, Hin: In oidx (c_l1_indices _), Host: _@[oidx] = Some _
+                   |- _] =>
+                  red in Hdiri; rewrite Forall_forall in Hdiri; specialize (Hdiri _ Hin);
+                  simpl in Hdiri; rewrite Host in Hdiri; simpl in Hdiri
+                end.
+                disc_InvL1DirI oidx0.
+                simpl; rewrite Hdiri; discriminate.
+            }
+            { apply NoCohMsgs_enq; [|solve_not_in].
+              eapply NoCohMsgs_rqDown_deq; eauto.
+            }
+          }
+          { eapply ObjsInvalid_l1_singleton; eauto; mred. }
+        }
+      }
+
+      { case_InvExcl_me_others.
+        { disc_InvExcl_this.
+          { solve_InvObjExcl0_by_ObjExcl0_false. }
+          { solve_InvObjOwned_by_false. }
+          { red; intros; exfalso; auto. }
+        }
+        { disc_InvExcl_others.
+          { disc_InvObjExcl0_apply.
+            split; [|solve_MsgsP].
+            solve_ObjsInvalid_trivial.
+            eapply ObjsInvalid_state_transition_sound; eauto.
+          }
+          { disc_InvObjOwned.
+            split; [|solve_MsgsP].
+            solve_ObjsInvalid_trivial.
+            eapply ObjsInvalid_state_transition_sound; eauto.
+          }
+          { split_InvDirInv_apply.
+            { case_in_subtree oidx cidx.
+              { solve_ObjsInvalid_trivial.
+                eapply ObjsInvalid_state_transition_sound; eauto.
+              }
+              { solve_ObjsInvalid_trivial. }
+            }
+            { case_in_subtree oidx cidx.
+              { solve_ObjsInvalid_trivial. }
+              { solve_ObjsInvalid_trivial.
+                eapply ObjsInvalid_state_transition_sound; eauto.
+              }
+            }
+          }
+        }
+      }
+    }
+
+    { (* [l1DownIImmME] *)
+      disc_rule_conds_ex.
+      derive_NoRsI_by_rqDown oidx msgs.
+
+      split.
+      { disc_MsgConflictsInv oidx.
+        solve_AtomicInv_rqDown_rsUp.
+        { simpl in *; inv H31; mred; simpl.
+          repeat split.
+          disc_InvL1DirI oidx0.
+          assumption.
         }
         { simpl in *; inv H31; mred.
           eapply ObjsInvalid_l1_singleton; eauto; mred.
@@ -6701,6 +7692,7 @@ Section InvExcl.
     { (* [l1InvRsDownDown] *)
       disc_rule_conds_ex.
       derive_footprint_info_basis oidx.
+      disc_InvL1DirI oidx.
 
       split.
       { solve_AtomicInv_rsDown. }
@@ -6718,9 +7710,9 @@ Section InvExcl.
             { solve_MsgsP. }
           }
           { case_InvObjOwned.
-            { left.
-              red; simpl; split; [solve_mesi|].
-              eapply NoCohMsgs_rsDown_deq; eauto.
+            { left; repeat split; [simpl; solve_mesi| |].
+              { simpl; rewrite Hdiri; discriminate. }
+              { eapply NoCohMsgs_rsDown_deq; eauto. }
             }
             { disc_ObjsInvalid_by oidx0.
               case_ObjInvalid; [solve_ObjInvalid0|solve_ObjInvRs].
@@ -6741,7 +7733,7 @@ Section InvExcl.
       }
     }
 
-    (* END_SKIP_PROOF_OFF *)
+    END_SKIP_PROOF_ON *) admit.
   Qed.
 
   Lemma mesi_InvExcl_InvTrs: InvTrs impl (InvExcl topo cifc).
