src/Ex/Mesi/MesiSim.v
@@ -85,7 +85,7 @@ Section Sim.
       - red in H; dest; repeat ssplit.
         + red; intros; solve_mesi.
         + do 2 red; intros.
-          specialize (H0 _ H1); red in H0.
+          specialize (H1 _ H2); red in H1.
           red; unfold cohMsgs, map, caseDec, fst in *.
           repeat (find_if_inside; [exfalso; auto; fail|]).
           destruct (sig_dec _ (_, (MRs, mesiRsM))); [exfalso; auto|].
@@ -487,7 +487,7 @@ Section Sim.
 
   Theorem mesi_sim_ok:
     InvSim step_m step_m (MesiInvOk.InvForSim tr) SimMESI impl spec.
-  Proof. (* SKIP_PROOF_OFF *)
+  Proof. (* SKIP_PROOF_ON
     red; intros.
 
     pose proof (footprints_ok
@@ -752,7 +752,18 @@ Section Sim.
         destruct (idx_dec lidx (obj_idx upCObj)); subst; solve_MsgsCoh.
       }
 
-      { (* [liDownIRsUpDown] *)
+      { (* [liDownIRsUpDownS] *)
+        disc_rule_conds_ex; spec_case_silent.
+        derive_footprint_info_basis oidx;
+          [|exfalso; subst topo; congruence].
+        derive_child_chns upCIdx.
+        derive_child_idx_in upCIdx.
+        disc_responses_from.
+        disc_rule_conds_ex.
+        solve_sim_mesi.
+      }
+
+      { (* [liDownIRsUpDownME] *)
         disc_rule_conds_ex; spec_case_silent.
         derive_footprint_info_basis oidx;
           [|exfalso; subst topo; congruence].
@@ -1069,7 +1080,7 @@ Section Sim.
         solve_sim_mesi.
       }
 
-      { (* [liDownIRsUpDown] *)
+      { (* [liDownIRsUpDownS] *)
         disc_rule_conds_ex; spec_case_silent.
         derive_footprint_info_basis oidx;
           [|disc_MesiDownLockInv oidx H29].
@@ -1080,7 +1091,27 @@ Section Sim.
         solve_sim_mesi.
       }
 
-      { (* [liDownIImm] *)
+      { (* [liDownIRsUpDownME] *)
+        disc_rule_conds_ex; spec_case_silent.
+        derive_footprint_info_basis oidx;
+          [|disc_MesiDownLockInv oidx H29].
+        derive_child_chns upCIdx.
+        derive_child_idx_in upCIdx.
+        disc_responses_from.
+        disc_rule_conds_ex.
+        solve_sim_mesi.
+      }
+
+      { (* [liDownIImmS] *)
+        disc_rule_conds_ex.
+        spec_case_silent.
+        assert (NoRsI oidx msgs)
+          by (solve_NoRsI_base; solve_NoRsI_by_rqDown oidx).
+        disc_rule_conds_ex.
+        solve_sim_mesi.
+      }
+
+      { (* [liDownIImmME] *)
         disc_rule_conds_ex.
         spec_case_silent.
         assert (NoRsI oidx msgs)
@@ -1100,7 +1131,15 @@ Section Sim.
         solve_sim_mesi.
       }
 
-      { (* [liDownIRsUpUp] *)
+      { (* [liDownIRsUpUpS] *)
+        disc_rule_conds_ex; spec_case_silent.
+        derive_footprint_info_basis oidx;
+          [disc_MesiDownLockInv oidx H29|].
+        disc_responses_from.
+        solve_sim_mesi.
+      }
+
+      { (* [liDownIRsUpUpME] *)
         disc_rule_conds_ex; spec_case_silent.
         derive_footprint_info_basis oidx;
           [disc_MesiDownLockInv oidx H29|].
@@ -1337,12 +1376,14 @@ Section Sim.
             solve_MsgsP.
           }
 
-      + (* [l1DownIImm] *)
+      + (* [l1DownIImmS] *)
         disc_rule_conds_ex.
         spec_case_silent.
-        assert (NoRsI oidx msgs)
-          by (solve_NoRsI_base; solve_NoRsI_by_rqDown oidx).
+        solve_sim_mesi.
+
+      + (* [l1DownIImmME] *)
         disc_rule_conds_ex.
+        spec_case_silent.
         solve_sim_mesi.
 
       + (* [l1InvRqUpUp] *)
@@ -1353,9 +1394,6 @@ Section Sim.
       + (* [l1InvRqUpUpM] *)
         disc_rule_conds_ex.
         spec_case_silent.
-        assert (NoRsI oidx msgs)
-          by (solve_NoRsI_base; solve_NoRsI_by_no_uplock oidx).
-        disc_rule_conds_ex.
         solve_sim_mesi.
 
       + (* [l1InvRsDownDown] *)
@@ -1368,7 +1406,7 @@ Section Sim.
         Unshelve.
         all: eassumption.
 
-        (* END_SKIP_PROOF_OFF *)
+        END_SKIP_PROOF_ON *) admit.
   Qed.
 
   Theorem mesi_ok:
