src/skip_proof.sh
@@ -6,7 +6,17 @@ if [[ "$PLATFORM" == 'Darwin' ]]; then
 	SED="$SED .orig"
 fi
 
-if [ "$1" = "-r" ]; then
+if [ "$1" = "-s" ]; then
+    file="$2";
+    echo "Setting SKIP_PROOF_ON in $file";
+    $SED -e 's/(\* SKIP_PROOF_OFF \*)/(\* SKIP_PROOF_ON/g' \
+	 -e 's/(\* END_SKIP_PROOF_OFF \*)/END_SKIP_PROOF_ON \*) admit\./g' "$file"
+elif [ "$1" = "-sr" ]; then
+    file="$2";
+    echo "Setting SKIP_PROOF_OFF in $file";
+    $SED -e 's/(\* SKIP_PROOF_ON/(\* SKIP_PROOF_OFF \*)/g' \
+	 -e 's/END_SKIP_PROOF_ON \*) admit\./(\* END_SKIP_PROOF_OFF \*)/g' "$file"
+elif [ "$1" = "-r" ]; then
 	for file in Ex/*/*.v;
 	do
 		echo "Setting SKIP_PROOF_OFF in $file"
